.. meta::
   :author: Shiv Shankar Dayal
   :title: Binomial Theorem
   :description: Algebra
   :keywords: Algebra, ratio, proportions, variations, complex numbers,
              arithmetic progressions, geometric progressions, harmonic
              progressions, series, sequence, quadratic equations,
              permutations, combinations, lograithms, binomial theorem,
              determinant, matrices

Binomials, Multinomials and Expansions Problems Part 4
******************************************************
151. Show that the number of permutations which can be formed from :math:`2n`
     letters which are either 'a' or 'b' is greatest when the number of
     a's is equal to the number of b.

152. Find the consecutive terms in the binomial expansion of :math:`(3 +
     2xy)^7` whose coefficients are equal.

153. Find the sum of coefficients in the expansion of :math:`(1 + 5x^2 -
     7x^3)^{2000}`

154. If the sum of the coefficients in the expansion of
     :math:`\left(3^{-\frac{x}{4}} + 3^{\frac{5x}{4}}\right)^n` is :math:`64`
     and the term with greatest coefficient exceeds the third term by :math:`(n
     - 1)` and :math:`[\alpha] = x,` where :math:`[\alpha]` denotes the
     integral part of :math:`\alpha` find the value of :math:`\alpha.`

155. Find the sum of coefficients in the expansion of the binomial coefficients
     :math:`(5p - 4q)^n,` where :math:`n` is a positive integer.

156. Find the sum of the coefficients of the polynomial :math:`(1 - 3x +
     x^3)^{201} . (1 + 5x - 5x^2)^{503}`

157. If the sum of the coefficients in the expansion of :math:`(tx^2 - 2x +
     1)^n` is equal to the sum of coefficients in the expansion of :math:`(x -
     ty)^n,` where :math:`n\in N,` then find the value of :math:`t.`

158. If :math:`a_0, a_1, a_2, \ldots, a_n` be the successive coefficient of
     :math:`(1 + x)^n,` show that

     :math:`(a_0 - a_2 + a_4 - \ldots)^2 + (a_1 -a_3 + a_5 - \ldots)^2 = a_0 +
     a_1 + \ldots + a_n = 2^n`

159. Find the greatest term in the expansion of :math:`\sqrt{3}\left(1 +
     \frac{1}{\sqrt{3}}\right)^{20}`

160. In the expansion :math:`(x + a)^{15},` if the eleventh term is the G.M. of
     the eightth and twelfth terms, which term in the expression is the
     greatest?

161. If the greatest term in the expansion of :math:`(1 + x)^{2n}` has the
     greatest coefficient if and only if :math:`x \in \left(\frac{10}{11},
     \frac{11}{10}\right)` and the fourth term in the expansion of
     :math:`\left(kx + \frac{1}{x}\right)^m,` is :math:`\frac{m}{4},` then find
     the value of :math:`mk.`

162. Given that the :math:`4^{th}` term in the exxpansion of :math:`\left(2 +
     \frac{3}{8}x\right)^{10}` has the maximum numerical value, find the range
     of values of :math:`x` for which this would be true.

163. If :math:`n` is a positive integer, show that :math:`9^n + 7` is divisible
     by :math:`8.`

164. If :math:`n` is a positive integer, show that :math:`3^{2n + 1} + 2^{n +
     2}` is divisible by :math:`7.`

165. Show that the roots of the equation :math:`ax^2 + 2bx + c = 0` are real
     and unequal, where :math:`a, b, c` are three consecutive coefficients in
     any binomial expansion with positive integral index.

166. Show that no three consecutive binomial coefficients can be in G.P. or
     H.P.

167. If :math:`(1 + x)^n = C_0 + C_1x + C_2x^2 + \ldots + C_nx^n,` show that
     :math:`C_n - 2.C_1 + 3.C_2 - \ldots +(-1)^n(n + 1)C_n = 0`

168. If :math:`(1 + x)^n = C_0 + C_1x + C_2x^2 + \ldots + C_nx^n,` show that
     :math:`C_0 -3.C_1 + 5.C_2 - \ldots + (-1)^n(2n + 1)C_n = 0`

169. If :math:`(1 + x)^n = C_0 + C_1x + C_2x^2 + \ldots + C_nx^n,` show that
     :math:`a - (a - 1)C_1 + (a - 2)C_2 - (a - 3)C_3 + \ldots + (-1)^n(a -
     n)C_n = 0`

170. Prove that :math:`\sum_{r = 0}^n r^2.{}^nC_r p^rq^{n - r} = npq + n^2p^2`
     if :math:`p + q = 1`

171. If :math:`C_r` stands for :math:`{}^nC_r,` show that :math:`2.C_0 +
     \frac{2^2}{2}C_1 + \frac{2^3}{3}C_2 + \ldots + \frac{2^{11}}{11}C_{11} =
     \frac{3^{11} - 1}{11}`

172. Prove that :math:`C_1 - \frac{1}{2}C_2 + \frac{1}{3}C_3 - \ldots +
     \frac{(1)^nC_n}{n} = 1 + \frac{1}{2} + \frac{1}{3} + \ldots + \frac{1}{n}`

173. Prove that :math:`\frac{C_0}{1} - \frac{C_1}{5} + \frac{C_2}{9} - \ldots +
     (-1)^n\frac{C_n}{4n + 1} = \frac{n.4^n}{1.5.9.\ldots (4n + 1)}`

174. Show that :math:`\frac{C_0}{n} - \frac{C_1}{n + 1} + \frac{C_2}{n + 2} -
     \ldots + (-1)^n\frac{C_n}{2n} = \frac{n!(n - 1)!}{(2n)!}`

175. Show that :math:`\frac{C_0}{n(n + 1)} - \frac{C_1}{(n + 1)(n + 2)} +
     \frac{C_2}{(n + 2)(n + 3)} - \ldots + (-1)^n\frac{C_{n}}{2n(2n + 1)} =
     \frac{1}{(2n + a)}.\frac{1}{{}^{2n}C_{n - 1}}`

176. Show that :math:`\frac{C_0}{x} - \frac{C_1}{x + 1} + \frac{C-2}{x + 2} -
     \ldots + (-1)^n\frac{C_n}{x + n} = \frac{n!}{x(x + 1)\ldots (x + n)}`

177. Show that :math:`C_0^2 - C_1^2 + C_2^2 - \ldots + (-1)^nC_n^2 = 0` or
     :math:`(-1)^{\frac{n}{2}}. \frac{n!}{\left(\frac{n}{2}\right)!}^2`
     according as :math:`n` is odd or even.

178. Show that :math:`{}^mC_r{}^nC_0 + {}^mC_{r - 1}{}^nC_1 + {}^mC_{r -
     2}{}^nC_2 + \ldots + {}^mC_0{}^nC_r = {}^{m + n}C_r,` where :math:`m, n,
     r` are positive integers and :math:`r < m, r < n.`

179. :math:`{}^{2n}C_0^2 - {}^{2n}C_1^2 + {}^{2n}C_2^2 - \ldots +
     (-1)^{2n}.{}^{2n}C_{2n}^2 = (-1)^n.{}^{2n}C_n.`

180. Show that :math:`C_1^2 + 2.C_2^2 + 3.C_3^2 + \ldots + n.C_n^2 =
     \frac{(2n - 1)!}{[(n - 1)!]^2}`

181. Show that :math:`C_0^2 + \frac{C_1^2}{2} + \frac{C_2^2}{3} + \ldots +
     \frac{C_n^2}{n + 1} = \frac{(2n + 1)!}{[(n + 1)!]^2}`

182. If :math:`n` is a positive integer in :math:`(1 + x)^n,` show that
     :math:`2.\frac{\left(\frac{n}{2}!\right)^2}{n!}[c_0^2 -2.C_1^2 + 3.C_2^2 -
     \ldots + (-1)^n.(n + 1)C_n^2] = (-1)^{\frac{n}{2}}(2 + n)`

183. Show that :math:`\sum_{0\leq i \leq n}\sum_{0\leq i \leq j\leq n}C_i
     C_j = 2^{2n - 1}- \frac{(2n)!}{2(n!)^2}`

184. Show that :math:`\sum_{r=0}^nC_r^3` is equal to the coefficient of
     :math:`x^ny^n` in the expansion of :math:`[(1 + x)(1 + y)(x + y)]^n.`

185. Let :math:`n` be a positive integer and :math:`(1 + x + x^2)^n = a_0 +
     a_1x + a_2x^2 + a_3x^3 + \ldots + a_{2n}x^{2n},` show that :math:`a_0^2 -
     a_1^2 + a_2^2 - \ldots + a_{2n}^2 = a_n`

186. Let :math:`n` be a positive integer and :math:`(1 + x + x^2)^n = a_0 +
     a_1x + a_2x^2 + a_3x^3 + \ldots + a_{2n}x^{2n},` show that :math:`a_0^2 -
     a_1^2 + a_2^2 - \ldots + (-1)^na_{n - 1}^2 = \frac{1}{2}a_n[1 -
     (-1)^na_n]`

187. Show that :math:`\sum_{0\leq i \leq n}\sum_{0\leq i \leq j\leq n} (C_i +
     C_j)^2 = (n - 1){}^{2n}C_n + 2^{2n}`

188. Show that :math:`\sum_{0\leq i \leq n}\sum_{0\leq i \leq j\leq n} (i +
     j)C_iC_j> = n(2^{2n - 1} - \frac{1}{2}{}^{2n}C_n)`

189. Show that :math:`(C_0 + C_1)(C_1 + C_2)(C_2 + C_3)\ldots (C_{n - 1} + C_n)
     = \frac{(n + 1)^n}{n!}C_1.C_2.\ldots .C_n`

190. If :math:`n` be a positive integer prove that :math:`\frac{1}{1!(n -
     1)!} + \frac{1}{3!(n - 3)!} + \frac{1}{5!(n - 5)! + \ldots + \frac{1}{(n -
     1)!1!}} = \frac{2^{n - 1}}{n!}`

191. Prove that :math:`\frac{3!}{2(n + 3)} =
     \sum_{r=0}^n(-1)^r.\left(\frac{{}^nC_r}{{}^{r + 3}C_r}\right)`

192. Show that for :math:`m\geq 2, C_0 - C_1 + C_2 - \ldots + (-1)^{m -
     1}C_{m - 1} = (-1)^{m - 1}\frac{(n- 1)(n - 2) \ldots (n - m + 1)}{(m -
     1)!}`

193. Find the GCD of :math:`{}^2nC_1, {}^{2n}C_3,{}^{2n}C_5, \ldots,
     {}^{2n}C_{2n - 1}`

194. Show that :math:`\sum_{r = 0}^n{}^nC_r \sin rx\cos (n  - r)x = 2^{n -
     1}\sin nx`

195. Show that :math:`C_1 -2.C_2 + 3.C_3 - \ldots + (-1)^{n - 1}n.C_n= 0`

196. :math:`a.C_0 + (a - b).C_1 + (a - 2b)C_2 + \ldots + (a - nb).C_n = 2^{n -
     1}(2a - nb)`

197. :math:`a^2.C_0 - (a - 1)^2.C_1 + (a - 2)^2.C_2 - \ldots + (-1)^n(a -
     n)^2.C_n = 0; n > 3`

198. If :math:`a_0, a_1, a_2, \ldots, a_n` be in an A.P, prove that
     :math:`a_0 - a_1.C_1 + a_2.C_2 - \ldots + (-1)^n a_n. C_n = 0`

199. Show that for :math:`n > 3, \sum_{r = 0}^n(-1)^r(a - r)(b - r)C_r = 0`

200. Show that for :math:`n > 3, \sum_{r = 0}^n(-1)^r(a - r)(b - r)(c - r)C_r =
     0`
