.. meta::
   :author: Shiv Shankar Dayal
   :title: Binomial Theorem
   :description: Algebra
   :keywords: Algebra, ratio, proportions, variations, complex numbers,
              arithmetic progressions, geometric progressions, harmonic
              progressions, series, sequence, quadratic equations,
              permutations, combinations, lograithms, binomial theorem,
              determinant, matrices

Binomials, Multinomials and Expansions Solutions Part 4
*******************************************************
151. This problem is similar to 149 and 150 and has been left as an exercise.

152. :math:`(3 + 2x)^7` will have :math:`8` terms with :math:`4^{th}` and
     :math:`5^{th}` terms as middle terms. We know that when there are two
     middle terms coefficients are equal. Therefore, these two middle terms are
     consecutive terms which have equal coefficient.

153. Let :math:`(1 + 5x^2 - 7x^3)^{2000} = a_0 + a_1x + a_2x + \ldots +
     a_{6000}x^{6000}`

     Substituting :math:`x = 1,` we get

     :math:`(1 + 5 - 7)^{2000} =` sum of coefficients :math:`= 1`

154. Substitutin :math:`x^{-\frac{x}{4}} = 1` and :math:`x^{\frac{5x}{4}} = 1`

     :math:`(1 + 1)^n = 64 \Rightarrow n = 6`

     Hence greatest term = middle term = :math:`4^{th}` term

     According to question :math:`t_4 = (n - 1)+ t_3`

     Solving this gives us, :math:`[\alpha] = 0`

155. Let :math:`S` be the sum of coeff. in :math:`(5p - 4q)^n`. Substituting
     :math:`p =1, q = 1,` we get

     :math:`S = (5 - 4)^n = 1`

156. Let :math:`S` be the sum of coeff. in :math:`(5p - 4q)^n`. Substituting
     :math:`x = 1,` we get

     :math:`S = (1 - 3 + 1)^{201}(1 + 5 - 5)^{503} = -1`

157. Substituing :math:`x =1` reduces the two expansions as  :math:`(t - 1)^n`
     and :math:`(1 - t)^n`

     Clearly, if :math:`n` is odd then sign will differe except when :math:`t =
     1.` However, if :math:`n` is even both expansions will be positive and
     :math:`t` can assume any real value.

158. Substituting :math:`x = 1, i, -i` and then multiplying when :math:`x = i,
     -i` we obtain the desired result.

159. Let :math:`r^{th}` term be the greatest term.

     :math:`t_r = \sqrt{3}\left[{}^{20}C_{r -
     1}\left(\frac{1}{\sqrt{3}}\right)^{r - 1}\right]`

     :math:`t_{r + 1} =
     \sqrt{3}\left[{}^{20}C_r\left(\frac{1}{\sqrt{3}}\right)^r\right]`

     :math:`\frac{t_r}{t_{r + 1}} = \frac{{}^{20}C_{r -
     1}}{{}^{20}C_r}\sqrt{r}`

     :math:`= \frac{r}{21 - r}\sqrt{3} \geq 1 \Rightarrow r = 7.69`

     Also, :math:`\frac{t_{r -1}}{t_r} \leq 1` gives us :math:`r = 8.5`

     Hence, :math:`8^{th}` term will be greatest term and :math:`t_8 =
     \frac{25840}{9}`

160. Since :math:`t_{11}` is G.M. of :math:`t_8` and :math:`t_{12}`

     :math:`t_{11} = \sqrt{t_8.t_{12}}`

     :math:`\left(\frac{15!}{10!5!}x^5a^{10}\right)^2 =
     \frac{15!15!}{7!8!11!4!}x^{12}a^{18}`

     :math:`\Rightarrow \frac{x}{a} = \sqrt{\frac{77}{75}}`

     Let :math:`r^{th}` term be the greatest term. Now,

     :math:`t_r = {}^{15}C_{r - 1}x^{16 - r}a^{r - 1}`

     :math:`t_{r + 1} = {}^{15C_r}x^{15 - r}a^r`

     :math:`\frac{t_r}{t_{r + 1}} = \frac{r}{16 - r}\frac{x}{a} \geq 1`

     :math:`r \geq 7.947`

     Hence, :math:`8^{th}` term is the greatest term.

161. :math:`t_{n + 1} = {}^{2n}C_nx^n, t_{n + 2} = {}^{2n}C_{n + 1}x^{n + 1},
     t_n = {}^{2n}C_{n - 1}x^{n - 1}`

     :math:`\frac{t_{n + 1}}}{t_{n + 2}} = \frac{n + 1}{n}.\frac{1}{x} > 1
     \Rightarrow x < \frac{n + 1}{n}`

     Also, :math:`t_{n + 1} = \frac{n + 1}{n}x > 1 \Rightarrow x > \frac{n}{n +
     1}`

     Thus, greatest term will have greatest coefficient if and only if :math:`x
     \in \left(\frac{n}{n + 1}, \frac{n + 1}{n}\right)`

     Given :math:`x \in \left(\frac{10}{11}, \frac{11}{10}\right)`

     Thus, :math:`n = 10`

     :math:`t_4 = \frac{n}{4} = \frac{5}{2}`

     :math:`\Rightarrow {}^{m}C_3(kx)^{m - 3}\frac{1}{x^3} = \frac{5}{2}`

     R.H.S. is independent of :math:`x, \Rightarrow m - 6 = 0, m = 6`

     :math:`{}^{6}C_3k^3 = \frac{5}{2}\Rightarrow k = \frac{1}{2}`

     :math:`\Rightarrow mk = 3`

162. This problem is similar to last problem and has been left as an
     exercise. The range is :math:`2 < x < \frac{64}{21}`

163. :math:`9^n + 7 = (8 + 1)^n + 7 = {}^nC_0.8^n + {}^nC_18{n - 1} + \ldots +
     {}^nC_{n - 1}8 + {}^nC_n + 7`

     :math:`= 8k + 1 + 7, k \in N = 8(k + 1)`

     Thus, the number is divisible by :math:`8`

164. Given expression is :math:`3^{2n + 1} + 2^{n + 2}` which can be rewritten
     as :math:`3.(7 + 2)^n + 4.2^n,` which upon expansion yields

     :math:`3({}^nC_07^n + {}^nC_17^{n - 1}2 + \ldots + {}^nC_n2^n) + 4.2^n`

     :math:`= 7k + 2^n(3 + 4), k \in N`

     The above expression is divisible by :math:`7.`

165. Let the binomial expansion be :math:`(x + y)^n` and :math:`a, b, c` be the
     coefficients of :math:`r^{th}, (r + 1)^{th}, (r + 2)^{th}` terms
     respectively.

     Then, :math:`a = {}^nC_{r - 1}, b = {}^nC_r, c = {}^nC_{r + 1}`

     The descriminant of given quadratic equation is :math:`D = b^2 - 4ac`

     Substituting values of :math:`a, b, c` and simplifying we obtain

     :math:`D = 4({}^nC_r)^2 \frac{n + 1}{(n - r + 1)(r + 1)}` where :math:`r`
     is non-negative integer.

     Clearly :math:`D > 0,` hence roots of given equation are real and unequal.

166. This problem is similar to previous one and has been left as an exercise.

167. **Calculus Method:**

     :math:`(1 + x)^n = C_0 + C_1x + C_2x^2 + \ldots + C_nx^n`

     Multiplying with :math:`x` and differentiating w.r.t. :math:`x,` we get

     :math:`(1 + x)^n + nx(1 + x)^{n - 1} = C_0 + 2xC_1 + 3x^2C_2 + (n +
     1)x^nC_n`

     Substituting :math:`x = -1,` we obtain

     :math:`C_n - 2.C_1 + 3.C_2 - \ldots +(-1)^n(n + 1)C_n = 0`

     **Second Method:**

     :math:`t_r = (-1)^{r - 1}r.{}^nC_{r - 1} = (-1)^{r - 1}(r- 1 +
     ).{}^nC_{r - 1} = (-1)^{r - 1}n.{}^{n - 1}C_{r - 2} + (-1)^{r -
     1}.{}^nC_{r - 1}`

     :math:`\sum_{r = 1}^{n + 1} = -n({}^{n - 1}C_0 - {}^{n - 1}C_1 + {}^{n -
     1}C_2 - \ldots + {-1}^{n - 1}.{}^{n - 1}C_{n - 1}) + ({}^nC_0 - {}^nC_1 +
     \ldots + (-1)^n.{}^nC_n)`

     :math:`= -n(1 - 1)^{n - 1} + (1 - 1)^n = 0`

168. **Calculus Method:**

     We know that :math:`(1 + x)^n = C_0 + C_1x + C_2x^2 + \ldots + C_nx^n`

     Substituting :math:`x = x^2` and multiplying with :math:`x,` we get

     :math:`x(1 + x^2)^n = C_0x + C_1.x^3 + C_2.x^5 + \ldots + (2n +
     1)x^{2n}.C_n`

     Differentiating both sides w.r.t :math:`x,` and substituting :math:`x =
     i,` we get

     :math:`C_0 -3.C_1 + 5.C_2 - \ldots + (-1)^n(2n + 1)C_n = (1 - 1)^n +
     i.n.(1 - 1)^{n - 1}.2i = 0`

     **Second Method:**

     :math:`t_r = = (-1)^{r - 1}(2r - 1).C_{r - 1} = (-1)^r[2(r - 1) +
     1]{}^nC_{r - 1}`

     :math:`= 2(-1)^{r - 1}.n{}^{n - 1}C_{r - 1} + (-1)^{r - 1}{}^nC_{r - 1}`

     :math:`\sum_{r = 1}^{n + 1}t_r = -2n[{}^{n - 1}C_0 - {}^{n - 1}C_1 +
     \ldots + (-1)^{n - 1}{}^{n - 1}C_{n - 1}] + [{}^{n}C_0 - {}^nC_1 +
     \ldots + (-1)^n{}^nC_n]`

     :math:`= -2n(1 - 1)^{n - 1} + (1 - 1)^n = 0`

169. **Calculus Method:**

     L.H.S. = :math:`a[C_0 - C_1 + C_2 - \ldots + (-1)^n.C_n] + [1.C_1 - 2C_2 +
     3.C_3 - \ldots + (-1)^n(-n)C_n]`

     :math:`= a(1 - 1)^n + 1.C_1 - 2C_2 + 3.C_3 - \ldots + (-1)^n(-n)C_n`

     Given, :math:`(1 + x)^n = C_0 + C_1x + C_2x^2 + \ldots + C_nx^n`

     Differentiating w.r.t. :math:`x` and  substuting :math:`x = -1,` we get

     :math:`1.C_1 - 2C_2 + 3.C_3 - \ldots + (-1)^n(-n)C_n = (1 - 1)^n = 0`

     Hence, desired equality is proved.

     **Second Method:**

     :math:`t_r = (-1)^{r - 1}[a - (r - 1)]{}^nC_{r -1}`

     :math:`= a(-1)^{r - 1}.{}^nC_{r - 1} - (-1)^{r - 1}n.{}^{n - 1}C_{r -1}`

     This can be proven to be :math:`0` like previous problems.

170. :math:`t_{r + 1} = r^r.{}^nC_rp^rq^{n - r}`

     :math:`= r.n.{}^{n - 1}C_{r - 1}p^rq^{n - r}`

     :math:`= n(r - 1 + 1){}^{n - 1}C_{r - 1}p^rq^{n - r}`

     :math:`= n[(n - 1).{}^{n - 2}C_{r - 2} + {}^{n  - 1}C_{r - 1}]p^rq^{n -
     r}`

     L.H.S. :math:`= \sum_{r = 0}^n t_{r + 1}`

     :math:`= n(n - 1)p^2\sum_{r = 0}^n {}^{n - 2}C_{r - 2}q^{n -2 - (r - 2)} +
     np\sum_{r = 0}^{n}{}^{n - 1}C_{r - 1}p^{r - 1}q^{n - 1 - (r - 1)}`

     :math:`= n(n - 1)p^2(p + q)^{n - 2} + np(p + q)^{n - 1}`

     :math:`= n(n - 1)p^2 + np [\because p + q = 1]`

     :math:`= n^2p^2 + npq`

171. :math:`(1 + x)^{10} = C_0 + C_1x + C_2x^2 + \ldots + C_10x^{10}`

     Integrating between limits :math:`0` and :math:`2` gives the desired result.

172. **Calculus Method:**

     :math:`(1 - x)^n = 1 - {}^nC_1x + {}^nC_2x^2 - \ldots + (-1)^{n - 1}{}^nC_nx^n`

     :math:`\frac{1 - (1 - x)^n}{x} = {}^nC_1 - {}^nC_2x + \ldots + (-1)^{n -
     1}C_{n}x^{n - 1} = \frac{x - (1 - x)^n}{x}`

     Integrating between limits :math:`0` and :math:`1,` we get

     :math:`\left[{}^nC_1x - {}^nC_2\frac{x^2}{2} + \ldots + (-1)^{n -
     1}\frac{x^n}{n}\right]_0^1 = \int_{0}^1\frac{1 - (1 - x)^n}{x}dx`

     Let :math:`z = 1 - x` then R.H.S. becomes :math:`\int_1^0 -\frac{1 - z^n}{1
     - z}dz`

     :math:`= \int_0^1(1 + z + z^2 + \ldots + z^{n - 1})dz`

     :math:`= \left[z + \frac{z^2}{2} + \ldots + \frac{z^n}{n}\right]_0^1`

     :math:`= 1 + \frac{1}{2} +\frac{1}{3} + \ldots + \frac{1}{n}`

     **Seccond Method:**

     Let :math:`S_n = C_1 - \frac{1}{2}C_2 + \frac{1}{3}C_3 - \ldots +
     \frac{(1)^nC_n}{n}`

     :math:`S_n = n - \frac{1}{2}\frac{n(n - 1)}{2!} + \frac{1}{3}\frac{n(n -
     1)(n - 2)}{3!} + \ldots`

     :math:`= (n - 1 + 1) - \frac{1}{2}\frac{(n - 1)(n - 2 + 2)}{2!} + \frac{(n
     - 1)(n - 2)(n - 3 + 3)}{3!} + \ldots`

     :math:`= S_{n - 1} + \frac{1}{n}\left[n - \frac{n(n - 1)}{2!} +
     \frac{n(n - 1)(n - 2)}{3!} + \ldots\right]`

     :math:`= S_{n - 1} - \frac{1}{n}[C_0 - C1 + C_2 + \ldots -1] = S_{n - 1} -
     \frac{1}{n}[(1 - 1)^n - 1]`

     :math:`S_{n - 1} + \frac{1}{n} \therefore S_n - S_{n - 1} = 1`

     Similarly :math:`S_{n - 1} - S_{n - 2} = \frac{1}{n - 2}`

     :math:`S_{n - 2} - S_{n - 3} = \frac{1}{n - 3}`

     :math:`\ldots`

     :math:`S_2 - S_1 = \frac{1}{3}`

     :math:`S_1 = 1`

     Adding we get :math:`S_n = 1 + \frac{1}{2} + \frac{1}{4} + \ldots +
     \frac{1}{n}`

173. :math:`(1 - x)^n = 1 - {}^nC_1x + {}^nC_2x^2 - \ldots + (-1)^{n -
     1}{}^nC_nx^n`

     Putting :math:`x = x^4,` and integrating between limits :math:`0` and
     :math:`1,` we get

     :math:`C_0 - \frac{C_1}{5} + \frac{C_2}{9} - \ldots +
     (-1)^n\frac{C_n}{4n + 1} = \int_{0}^1(1 - x^4)^ndx`

     It can be proven that :math:`\int_0^1(1 - x^4)^ndx =
     \frac{4n.n!}{1.5.9\ldots (4n + 1)}` [Refer to any book on calculus]

174. :math:`(1 - x)^n = 1 - {}^nC_1x + {}^nC_2x^2 - \ldots + (-1)^{n -
     1}{}^nC_nx^n`

     Multiplying both sides with :math:`x^{n - 1},` and integrating with limit
     :math:`0` and :math:`1,` we get

     :math:`\frac{C_0}{n} - \frac{C_1}{n + 1} + \frac{C_2}{n + 2} -
     \ldots + (-1)^n\frac{C_n}{2n} = \int_0^1 x^{n - 1}(1 - x)^ndx`

     Integrating R.H.S. by parts we obtain the desired result.

175. L.H.S. :math:`= \left(\frac{C_0}{n} - \frac{C_0}{n + 1}\right) -
     \left(\frac{C_1}{n + 1} - \frac{C_1}{n + 2}\right) + \ldots + (-1)^{n -
     1}\left(\frac{C_n}{2n} - \frac{C_n}{2n + 1}\right)`

     :math:`= \left(\frac{C_0}{n} - \frac{C_1}{n + 1} + \frac{C_2}{n + 2} -
     \ldots + (-1)^n\frac{C_n}{2n}\right) - \left(\frac{C_0}{n + 1} -
     \frac{C_1}{n + 2} + \ldots + (-1)^n\frac{C_n}{2n + 1}\right)`

     Now this can be solved like 174.

176. This problem is similar to 174 and has been left as an exercise.

177. :math:`(1 + x)^n = C_0 + C_1x + C_2x^2 + \ldots + C_nx^n`

     :math:`(1 - x)^n = 1 - {}^nC_1x + {}^nC_2x^2 - \ldots + (-1)^{n -
     1}{}^nC_nx^n`

     Multiplying these two we get

     :math:`(C_0 + C_1x + C_2x^2 + \ldots + C_nx^n)(1 - {}^nC_1x + {}^nC_2x^2 -
     \ldots + (-1)^{n - 1}{}^nC_nx^n) = (1 - x^2)^n`

     Coeff. of :math:`x^n` on L.H.S. :math:`= C_0^2 - C_1^2 + C_2^2 - \ldots +
     (-1)^nC_n^2`

     R.H.S. :math:`= C_0 + (-1)^1C_1x^2 + C_2x^2 + \ldots`

     :math:`=` an expression having even powers of :math:`x`

     Thus, if :math:`n` is odd, coeff. of :math:`x^n` on R.H.S :math:`= 0`

     If :math:`n` is even, coeff. of :math:`x^n` on R.H.S. :math:`=
     (-1)^{\frac{n}{2}}{}^nC_{\frac{n}{2}}`

     :math:`= \frac{n!}{\left(\frac{n!}{2}\right)^2}`

178. :math:`(1 + x)^n = C_0 + C_1x + C_2x^2 + \ldots + C_nx^n`X

     :math:`(1 + x)^m = C_0 + C_1x + C_2x^2 + \ldots + C_mx^m`

     Multiplying these two, we get

     :math:`(C_0 + C_1x + C_2x^2 + \ldots + C_nx^n)(C_0 + C_1x + C_2x^2 +
     \ldots + C_mx^m) = (1 + x)^{m + n} = {}^{m + n}C_0 + {}^{m + n}C_1x +
     \ldots + {}^{m + n}C_rx^r + \ldots + {}^{m + n}C_{m + n}x^{m + n}`

     Equating the coefficient of :math:`x^r` we get the desired result.

179. :math:`(1 + x)^{2n} = C_0 + C_1x + C_2x^2 + \ldots + C_{2n}x^{2n}`

     :math:`(x + 1)^{2n} = C_0x^{2n} + C_1x^{2n - 1} + C_2x^{2n - 2} + \ldots +
     C_2n`

     Multiplying we get

     :math:`(C_0 + C_1x + C_2x^2 + \ldots + C_{2n}x^{2n})(C_0x^{2n} + C_1x^{2n - 1} +
     C_2x^{2n - 2} + \ldots + C_{2n}) = (1 - x^2)^{n}`

     Equating the coefficients of :math:`x^{2n}` we get the desired result.

180. :math:`(1 + x)^n = C_0 + C_1x + C_2x^2 + \ldots + C_nx^n`

     Differentaiating w.r.t :math:`x,` we obtain

     :math:`n(1 + x)^{n - 1} = C_1 + 2C_2x + \ldots + nC_nx^{n -1}`

     Also, :math:`(x + 1)^n = C_0x^n + C_1x^{n - 1} + C_2x^{n - 2} + \ldots +
     C_n`

     Multiplying two previous equations, we obtain

     :math:`n(1 + x)^{2n - 1} = (C_1 + 2C_2x + \ldots + nC_nx^{n -1})(C_0x^n +
     C_1x^{n - 1} + C_2x^{n - 2} + \ldots + C_n)`

     Equating coefficients of :math:`x^{n - 1},` we obtain

     :math:`C_1^2 + 2.C_2^2 + 2.C_3^3 + \ldots + n.C_n^2 = n.{}^{2n - 1}C_{n -
     1} = \frac{(2n - 1)!}{[(n - 1)!]^2}`

181. :math:`(1 + x)^n = C_0 + C_1x + C_2x^2 + \ldots + C_nx^n`

     Integrating with limits :math:`0` and :math:`x,` we obtain

     :math:`\left[\frac{(1 + x)^{n + 1}}{n + 1}\right]_0^x = \left[C_0x +
     C_1\frac{x^2}{2} + C_2\frac{x^3}{3} + \ldots + C_n\frac{x^{n + 1}}{n +
     1}\right]_0^x`

     Also, :math:`(x + 1)^n = C_0x^n + C_1x^{n - 1} + C_2x^{n - 2} + \ldots +
     C_n`

     Multiplying and equating coefficients of :math:`x^{n + 1},` we obtain

     :math:`C_0^2 + \frac{C_1^2}{2} + \frac{C_2^2}{3} + \ldots + \frac{C_n^2}{n
     + 1} = \frac{{}^{2n + 1}C_{n + 1} - 0}{n + 1} = \frac{(2n + 1)!}{[(n + 1)!]^2}`

182. :math:`(1 - x)^n = C_0 - C_1x + C_2x^2 - \ldots + (-1)^nC_nx^n`

     Multiplying with :math:`x,` we obtain

     :math:`x(1 - x)^n = C_0x + C_1x^2 + \ldots + (-1)^nC_nx^n`

     Differentiating w.r.t :math:`x,` we get

     :math:`(1 - x)^n - nx(1 - x)^{n - 1} = C_0 -2xC_1 + \ldots + (-1)^n(n + 1)x^nC_n`

     Again :math:`(x + 1)^n = C_0x^n + C_1x^{n - 1} + \ldots + C_0`

     Multiplying last two equations and equating coefficients of :math:`x^n`, we get

     :math:`C_0^2 -2.C_^2 + 3.C_2^2 - \ldots + (-1)^n(n + 1)C_n^2 = (1 - x^2)^n -nx(1 - x^2)^{n - 1} - nx^2(1 - x^2)^{n - 1}`

     :math:`= (-1)^{\frac{n}{2}}{}^nC_\frac{n}{2} - (-1)^{\frac{n}{2} - 1}.n{}^{n - 1}C_{\frac{n}{2} - 1}`

     :math:`= (-1)^\frac{n}{2}\frac{n!}{\left(\frac{n}{2}\right)!\left(\frac{n}{2}\right)!}\left(\frac{2 + n}{2}\right)`

183. :math:`2\sum_{0\leq i \leq n}\sum_{0\leq i \leq j\leq n}C_i C_j = (C_0 + C_1 + \ldots C_n)^2 - (C_0^2 + C_1^2 + \ldots +
     C_n^2)`

     :math:`= (2^n)^2 - {}^{2n}C_n`

     :math:`\Rightarrow \sum_{0\leq i \leq n}\sum_{0\leq i \leq j\leq n}C_i C_j = 2^{2n - 1} - \frac{(2n)!}{2(n!)^2}`

184. :math:`(1 + x)^n(y + 1)^n(x + y)^n = (C_0 + C_1x + \ldots + C_nx^n)(C_0y^n + C_1y^{n - 1} + \ldots + C_n)(C_0x^n + C_1x^{n -
     1}y + \ldots + C_ny^n)`

     Coeff. of :math:`x^ny^` in L.H.S. :math:`= C_0^3 + C_1^3 + C_2^3 + \ldots + C_n^3`

185. Given :math:`(1 + x + x^2)^n = a_0 + a_1x + a_2x^2 + a_3x^3 + \ldots + a_{2n}x^{2n}`

     Putting :math:`x^2` in place of :math:`x,` we get

     :math:`(1 + x^2 + x^4) = a_0 + a_1x^2 + a_2x^4 + \ldots + a_nx^{2n} + \ldots + a_{2n}x^{4n}`

     Coeff. of :math:`x^{2n} = a_n`

     Putting :math:`-\frac{1}{x}` in place of :math:`x,` we get

     :math:`\left(1 - \frac{1}{x} + \frac{1}{x^2}\right)^n = a_0 - a_1\frac{1}{x} + a_2\frac{1}{x^2} + \ldots +
     a_{2n}\frac{1}{x^{2n}}`

     :math:`(x^2 - x + 1)^n = a_0x^{2n} - a_1x^{2n - 1} + \ldots + a_{2n}`

     :math:`\therefore (1 + x + x^2)^n(x^2 -x + 1)^n = (a_0 + a_1x + a_2x^2 + a_3x^3 + \ldots + a_{2n}x^{2n})(a_0 - a_1\frac{1}{x} +
     a_2\frac{1}{x^2} + \ldots + a_{2n}\frac{1}{x^{2n}})`

     Equating coeff. of :math:`x^{2n},` we obtain

     :math:`a_0^2 - a_1^2 + a_2^2 - \ldots + a_{2n}^2 = a_n`

186. Given :math:`(1 + x + x^2)^n = a_0 + a_1x + a_2x^2 + a_3x^3 + \ldots + a_{2n}x^{2n}`

     Putting :math:`-\frac{1}{x}` in place of :math:`x,` we get

     :math:`\left(1 - \frac{1}{x} + \frac{1}{x^2}\right)^n = a_0 - a_1\frac{1}{x} + a_2\frac{1}{x^2} + \ldots +
     a_{2n}\frac{1}{x^{2n}}`

     :math:`(x^2 - x + 1)^n = a_0x^{2n} - a_1x^{2n - 1} + \ldots + a_{2n}`

     :math:`\therefore (1 + x + x^2)^n(x^2 -x + 1)^n = (a_0 + a_1x + a_2x^2 + a_3x^3 + \ldots + a_{2n}x^{2n})(a_0 - a_1\frac{1}{x} +
     a_2\frac{1}{x^2} + \ldots + a_{2n}\frac{1}{x^{2n}})`

     :math:`(1 + x^2 + x^4)^n = a_0 + a_1x^2 + a_2x^4 + \ldots + a_{2n}x^{4n}`

     Equating coff. of :math:`x^{2n}` from both sides, we obtain

     :math:`a_0^2 - a_1^2 + a_2^2 - \ldots + a_{2n}^2 = a_n`

     Putting :math:`x = \frac{1}{x}` in origina equation

     :math:`(x^2 + x + 1)^n = a_0x^{2n} + a_1x^{2n - 1} + \ldots + a_{2n}`

     Equating coff. of equal powers of :math:`x,` we obtain

     :math:`a_0 = a_{2n}, a_1 = a_{2n - 1} , \ldots a_{n - 1} = a_{n + 1}`

     We have obtained

     :math:`a_0^2 - a_1^2 + a_2^2 - \ldots + (-1)^{n - 1}a_n^2 + (-1)^na_n^2 + (-1)^{n + 1}a_{n + 1}^2 + \ldots + (-1)^{2n}a_{2n}^2
     = a_n`

     :math:`2(a_0^2 - a_1^2 + a_2^2 - \ldots + (-1)^{n - 1}a_n^2) = a_n - (-1)^na_n^2`

     :math:`a_0^2 - a_1^2 + a_2^2 - \ldots + (-1)^{n - 1}a_n^2 = \frac{1}{2}a_n[1 - (-1)^na_n]`

187. Let :math:`x = \sum_{0\leq i \leq n}\sum_{0\leq i \leq j\leq n} (C_i + C_j)^2`

     :math:`x = n(C_0^2 + C_1^2 + \ldots C_n^2) + 2\sum_{0\leq i \leq n}\sum_{0\leq i \leq j\leq n}C_i C_j`

     Making use of results from 183

     :math:`= n.{}^{2n}C_n + (C_0 + C_1 + C_2 + \ldots + C_n)^2 - (C_0^2 + C_1^2 + \ldots C_n^2)`

     :math:`= (n - 1){}^2nC_n + 2^{2n}`

188. Let :math:`x = \sum_{0\leq i \leq n}\sum_{0\leq i \leq j\leq n} (i + j)C_iC_j`

     Here :math:`i = 0, 1, 2, 3, \ldots, (n - 1),` and :math:`j = 1, 2, 3, \ldots, n`

     Clearly, :math:`n - i = n, n - 1, n - 2, \ldots, 1` and :math:`n - j = n - 1, n- 2, \ldots, 0`

     We observe that :math:`n - j` has same values as :math:`i` and :math:`n - i` has same values as :math:`j.

     Hence replacing :math:`j` by :math:`n - i` and :math:`i` by :math:`n - j,` we obtain

     :math:`x = \sum_{0\leq i \leq n}\sum_{0\leq i \leq j\leq n} (n - j + n - i){}^nC_{n - j}{}^nC_{n - i}`

     :math:`= 2n \sum_{0\leq i \leq n}\sum_{0\leq i \leq j\leq n}C_i C_j - \sum_{0\leq i \leq n}\sum_{0\leq i \leq j\leq n}(i +
     j)C_iC_j`

     :math:`2x = 2. n\sum_{0\leq i \leq n}\sum_{0\leq i \leq j\leq n}C_iC_j`

     :math:`2x = n[(C_0 + C_1 + \ldots + C_n)^2 - (C_0^2 + C_1^2 + \ldots + C_n^2)]`

     :math:`x=n(2^{2n - 1} - \frac{1}{2}{}^{2n}C_n)`

189. :math:`r^{th}` factor of L.H.S. is given by

     :math:`t_r = {}^nC_{r - 1} + {}^nC_r = \frac{n + 1}{r}{}^nC_{r - 1}`

     Thus, L.H.S. :math:`= \left(\frac{n + 1}{1}{}^nC_0\right).\left(\frac{n + 1}{2}{}^nC_1\right)\ldots \left(\frac{n +
     1}{n}{}^nC_{n - 1}\right)`

     :math:`= \frac{(n + 1)^n}{n!}C_1C_2C_3\ldots C_n`

190. L.H.S. :math:`= \frac{1}{n!}\left[\frac{n!}{1!(n - 1)!} + \frac{n!}{3!(n - 3)!} + \ldots + \frac{n!}{(n - 1)!1!}\right]`

     :math:`= \frac{1}{n!}[C_1 + C_3 + \ldots + C_{n - 1}]`

     :math:`= \frac{1}{n!}2^{n - 1}`

191. R.H.S. :math:`= \sum_{r=0}^n(-1)^r.\left(\frac{{}^nC_r}{{}^{r + 3}C_r}\right)`

     :math:`= \sum_{r=0}^n(-1)^r \frac{n!}{r!(n - r!)}.\frac{r!3!}{(r + 3)!}`

     :math:`= 3!\sum_{r=0}^n(-1)^r \frac{n!}{(n - r)!(r + 3)!}`

     :math:`= \frac{3!}{(n + 1)(n + 2)(n + 3)}\sum_{r=0}^n(-1)^r \frac{(n + 3)!}{(r + 3)!(n - r)!}`

     :math:`= \frac{3!}{(n + 1)(n + 2)(n + 3)}\sum_{r=0}^n(-1)^r {}^{n + 3}C_{r + 3}`

     :math:`= \frac{3!}{(n + 1)(n + 2)(n + 3)}[{}^{n + 3}C_3 - {}^{n + 3}C_4 + \ldots + (-1)^n.{}^{n + 3}C_{n + 3}]`

     :math:`\because {}^{n + 3}C_0 - {}^{n + 3}C_1 + \ldots + (-1)^{n + 3}.{}^{n + 3}C_{n + 3} = 0`

     :math:`\therefore {}^{n + 3}C_3 - {}^{n + 3}C_4 + \ldots + (-1)^n.{}^{n + 3}C_{n + 3} = {}^{n + 3}C_0 - {}^{n + 3}C_1 + {}^{n +
     3}C_2`

     :math:`= \frac{(n + 1)(n + 2)}{2}`

     Now we can easily prove the required equality.

192.
