.. meta::
   :author: Shiv Shankar Dayal
   :title: Binomial Theorem
   :description: Algebra
   :keywords: Algebra, ratio, proportions, variations, complex numbers,
              arithmetic progressions, geometric progressions, harmonic
              progressions, series, sequence, quadratic equations,
              permutations, combinations, lograithms, binomial theorem,
              determinant, matrices

Binomials, Multinomials and Expansions Problems Part 5
******************************************************
201. Find the value of :math:`n` for :math:`\frac{C_0}{2^n} + \frac{2.C_1}{2^n}
     + \frac{3.C_2}{2^n} + \ldots + \frac{(n + 1)C_n}{2^n} = 16` is true?

202. If :math:`a_0, a_1, a_2, \ldots, a_{n + 1}` be in an A.P, prove that
     :math:`\sum_{k = 0}^n a_{k + 1}C_k = 2^{n - 1}(a_1 + a_{n + 1})`

203. If :math:`s = \frac{n + 1}{2}[2a + nd]` and :math:`S = a + (a + d)C_1 +
     (a + 2d)C_2 + \ldots + (a + nd)C_n,` prove that :math:`(n + 1)S = 2^n.s`

204. If :math:`(1 + x + x^2 + \ldots + x^p)^n = a_0 + a_1x + a_2x^2 + \ldots +
     a_{np}x^{np},` show that :math:`a + 2a_2 + 3a_3 + \ldots + npa_{np} =
     \frac{1}{2}np(p + 1)^n`

205. Prove that :math:`C_0 - 2^2C_1 + 3^2 C_2 - \ldots + (-1)^n(n + 1)^2C_n =
     0, n > 2`

206. Show that :math:`\frac{C_1}{2} + \frac{C_3}{4} + \frac{C_5}{6} + \ldots =
     \frac{2^n - 1}{n + 1}`

207. Show that :math:`\frac{C_0}{1.2} - \frac{C_1}{2.3} + \frac{C_2}{3.4} +
     \ldots + (-1)^n\frac{C_n}{(n + 1)(n + 2)} = \frac{1}{n + 2}`

208. Show that :math:`\frac{C_0}{2} - \frac{C_1}{3} + \frac{C_2}{4} - \ldots +
     (-1)^n\frac{C_n}{n + 2} = \frac{1}{(n + 1)(n + 2)}`

209. Show that :math:`\frac{C_0}{3} - \frac{C_1}{4} + \frac{C_2}{5} - \ldots +
     (-1)^n\frac{C_n}{n + 3} = \frac{2}{(n + 1)(n + 2)(n + 3)}`

210. Show that :math:`3.C_0 + 3^2\frac{C_1}{2} + 3^3\frac{C_2}{3} + \ldots +
     3^{n + 1}\frac{C_n}{n + 1} = \frac{4^{n + 1} - 1}{n + 1}`

211. Show that :math:`\sum_{k = 0}^{15}\frac{{}^{15}C_k}{(k + 1)(k + 2)} =
     \frac{2^{17} - 18}{16.17}`

212. Show that :math:`\frac{C_0}{1} - \frac{C_1}{4} + \frac{C_2}{7} - \ldots +
     (-1)^n\frac{C_n}{3n + 1} = \frac{3^nn!}{1.4.7.\ldots + (3n + 1)}`

213. Show that :math:`\sum_{r = 0}^n \frac{(-1)^rC_r}{(r + 1)(r + 2)} =
     \frac{1}{n + 2}`

214. Prove that :math:`\sum_{r = 0}^n \frac{C_r3^{r + 3}}{(r + 1)(r + 2)(r +
     3)} = \frac{4^{n + 3} - 1 - \frac{3}{2}(n + 3)(3n + 8)}{(n + 1)(n + 2)(n +
     3)}`

215. Prove that :math:`\sum_{r = 0}^n \frac{r + 2}{r + 1}C_r = \frac{2^n(n + 3)
     - 1}{n + 1}`

216. Show that :math:`\sum_{r = 0}^n \frac{3^{r + 4}C_r}{(r + 1)(r + 2)(r +
     3)(r + 4)} = \frac{1}{(n + 1)(n + 2)(n + 3)(n + 4)}\left[4^{n + 4} -
     \sum_{k = 0}^3 {}^{n + 4}C_k3^k\right]`

217. Show that :math:`\sum_{r=0}^{n - 3}C_rC_{r + 3} = \frac{(2n)!}{(n +
     3)!(n - 3)!}`

218. Show that sum of the product taken two at a time from :math:`C_0, C_1,
     C_2, \ldots` is :math:`2^{2n - 1}\frac{(2n - 1)!}{n!(n - 1)!}`

219. If :math:`S_n = C_0C_1 + C_1C_2 + \ldots + C_{n - 1}C_n` and
     :math:`\frac{S_{n + 1}}{S_n} = \frac{15}{4},` find n.

220. Show that :math:`C_0^2 + \frac{C_1^2}{2} + \frac{C_2^2}{3} + \ldots +
     \frac{C_n^2}{n + 1} = \frac{(n + 2)(2n - 1)!}{n!(n - 1)!}`

221. Show that :math:`C_1^2 -2.C_2^2 + 3.C_3^2 - \ldots - 2nC_{2n}^2 = (-1)^{n -
     1}.n.C_n` where :math:`C_r = {}^{2n}C_r`

222. Show that :math:`{}^{25}C_0^2 - {}^{25}C_1^2 + {}^{25}C_2^2 - \ldots -
     {}^{25}C_25^2 = 0`

223. Show that :math:`C_0.{}^{2n}C_n - C_1{}^{2n - 2}C_n + C_2{}^{2n -4}C_n -
     \ldots = 2^n`

224. Show that :math:`\sum_{0\leq i \leq n}\sum_{0\leq i \leq j\leq n}(i +
     j)(C_i + C_j + C_iC_j) = n^2.2^n + n\left(2^{2n - 1} -
     \frac{(2n)!}{2(n!)^2}\right)`

225. If :math:`(1 + x + x^2)^n = a_0 + a_1x + a_2x^2 + \ldots + a_{2n}x^{2n}`
     show that :math:`a_0a_{2r} - a_1a_{2r + 1} + a_2a_{2r + 2} - \ldots +
     a_{2n -2r}a_{2n} = a_{n + r}`

226. If :math:`a_r = \frac{1.3.5.\ldots (2r - 1)}{2.4.6.\ldots 2r}` then show
     that :math:`a_{2n + 1} + a_1a_{2n} + a_2a_{2n - 1} + \ldots +
     a_na_{n + 1} = \frac{1}{2}`

227. If :math:`P_n` denotes the product of all coefficients in the expansion of
     :math:`(1 + x)^n,` show that :math:`\frac{P_{n + 1}}{P_n} = \frac{(n +
     1)^n}{n!}`

228. Show that :math:`\sum_{r = 1}^nr^3\left(\frac{C_r}{C_{r - 1}}\right)^2 =
     \frac{1}{12}n(n + 1)^2(n + 2)`

229. Show that :math:`C_3 + C_7 + C_11 + \ldots = \frac{1}{3}\left[2^{n - 1}
     -2^{\frac{n}{2}}\sin \frac{n\pi}{4}\right]`

230. If :math:`(1 + x + x^2)^{20} = a_0 + a_1x + a_2x^2 + \ldots +
     a_{40}x^{40},` then find the value of :math:`a_0 + a_2 + a_4 + \ldots +
     a_{40}`

231. If :math:`(1 + x + x^2)^{20} = a_0 + a_1x + a_2x^2 + \ldots +
     a_{40}x^{40},` then find the value of :math:`a_1 + a_3 + a_5 + \ldots +
     a_{39}`

232. Show that :math:`C_1 - \frac{C_2}{2} + \frac{C_3}{3} - \ldots +
     (-1)^n\frac{C_n}{n} + \frac{1}{n(n - 1)} + \frac{2}{(n - 1)(n - 2)} +
     \ldots + \frac{n - 2}{2.3} = \frac{n + 1}{2}`

233. Show that :math:`\sum_{0\leq i \leq n}\sum_{0\leq i \leq j\leq n}
     \frac{i}{C_i + \frac{j}{C_j}} = \frac{n^2}{2}\sum_{r = 0}^n \frac{1}{C_r}`

234. Show that :math:`\sum_{0\leq i \leq n}\sum_{0\leq i \leq j\leq n}
     i.j.C_i.C_j = n^2\left[2^{2n - 3} - \frac{1}{2}{}^{2n - 2}C_{n -
     1}\right]`

235. Prove that :math:`C_1 - \left(1 + \frac{1}{2}\right)C_2 + \left(1 +
     \frac{1}{2} + \frac{1}{3}\right)C_3 - \ldots + (-1)^n\left(1 + \frac{1}{2}
     + \ldots + \frac{1}{n}\right)C)n = \frac{1}{n}`

236. Find the coefficient of :math:`x^5` in the expansion of :math:`(1 + 2x +
     3x^2)^4`

237. Find the coefficient of :math:`x^3y^4z^2` in the expansion of :math:`(2x -
     3y + 4z)^9`

238. Find the number of terms in :math:`(2x - 3y + 4z)^{100}`

239. Find the coefficient of :math:`x^4` in the expansion of :math:`(1 + x +
     x^2)^3`

240. Find the coefficient of :math:`x^{10}` in :math:`(1 + x + x^2 + x^3 +
     x^4 + x^5)^3`

241. Find the coefficient of :math:`x^7` in :math:`(1 + 3x - 2x^3)^{10}`

242. Find the coefficient of :math:`x^3y^4z^5` in :math:`(xy + yz + zx)^6`

243. Find the greatest coefficient in :math:`(w + x + y + z)^{15}`

244. Find the number of terms in :math:`(a + b + c + d + e)^{100}`

245. If :math:`|x| < 1,` show that :math:`(1 + x)^{-2} = 1 + 2x + 3x^2 + 4x^3 +
     \ldots ~\text{to}~\infty`

246. Find :math:`a, b` so that the coefficient of :math:`x^n` in the
     expansionof :math:`\frac{(a + bx)}{(1 - x)^2}` may be :math:`2n + 1` and
     hence find the sum of the series :math:`1 + 3\left(\frac{1}{2}\right) +
     5\left(\frac{1}{2}\right)^2 + \ldots`

247. Sum the series :math:`1 + \frac{1}{3} + \frac{1.3}{3.6} +
     \frac{1.3.5}{3.6.9} + \ldots~\text{to}~\infty`

248. If :math:`|x| <1,` show that :math:`(1 - x)^{-1} = 1 + x + x^2 + x^3 +
     \ldots~\text{to}~\infty`

249. If :math:`|x| <1,` show that :math:`(1 + x)^{-1} = 1 - x + x^2 - x^3 +
     \ldots~\text{to}~\infty`

250. If :math:`|x| <1,` show that :math:`(1 + x)^{-2} = 1 - 2x + 3x^2 - 4x^3 +
     \ldots~\text{to}~\infty`
