Determinants Problems Part 4
****************************
151. For positive numbers :math:`x, y , z` (not equal to :math:`1`), show that
     the numerical value of the determinant

     :math:`\begin{vmatrix}1 & \log_xy & \log_xz \\ \log_yx & 1 & \log_yz
     \\ \log_zx & \log_zy & 1\end{vmatrix} = 0`

152. If :math:`a, b, c > 0` and :math:`x, y , z \in R,` then show without
     expanding that

     :math:`\begin{vmatrix}(a^x + a^{-x})^2 & (a^x - a^{-x})^2 & 1 \\ (b^y +
     b^{-y})^2 & (b^y - b^{-y})^2 & 1 \\ (c^z + c^{-z})^2 & (c^z - c^{-z})^2 &
     1\end{vmatrix} = 0`

153. Wihtout expanding the determinants prove that

     :math:`\begin{vmatrix}103 & 115 & 114 \\ 111 & 108 & 106 \\ 104 & 113 &
     116\end{vmatrix} + \begin{vmatrix}113 & 116 & 104 \\ 108 & 106 & 111 \\
     115 & 114 & 103\end{vmatrix} = 0`

154. Evaluate :math:`\sum_{n = 1}^N U_n` if :math:`U_n = \begin{vmatrix}n & 1 &
     5 \\ n^2 & 2N + 1 & 2N+ 1 \\ n^3 & 3N^2 & 3N\end{vmatrix}`

155. If :math:`A, B, C` are angles of a triangle, then show without expanding
     that

     :math:`\begin{vmatrix}\sin(A + B + C) & \sin B & \cos C \\ -\sin B & 0 &
     \tan A \\ \cos (A + B) & -\tan A & 0\end{vmatrix} = 0`

156. Evaluate without expanding :math:`\begin{vmatrix}b^2 - ab & b - c & bc -
     ac \\ ab - a^2 & a - b & b^2 -a b \\ bc - ac & c - a & ab -
     a^2\end{vmatrix}`

157. Let :math:`\Delta_i = \begin{vmatrix}i - 1 & n & 6 \\ (i - 1)^2 & 2n^2 &
     4n - 2 \\ (i - 1)^3 & 3n^3 & 3n^2 - 2n\end{vmatrix}`

     Show that :math:`\sum_{i = 1}^n \Delta_i = k,` a constant.

158. Let :math:`m` be a positive integer and :math:`\Delta_r =
     \begin{vmatrix}2r - 1 & {}^mC_r & 1 \\ m^2 - 1 & 2^m & m + 1 \\
     \sin^2m^2\ & \sin^2 m & \sin^2(m + 1) \end{vmatrix}`

     Then find the value of :math:`\sum_{r = 0}^m\Delta_r`

159. Show that :math:`\begin{vmatrix}{}^xC_r & {}^xC_{r + 1} & {}^xC_{r + 2} \\
     {}^yC_r & {}^yC_{r + 1} & {}^yC_{r + 2} \\ {}^zC_r & {}^zC_{r + 1} &
     {}^zC_{r + 2} \end{vmatrix} = \begin{vmatrix}{}^xC_r & {}^{x + 1}C_{r + 1}
     & {}^{x + 2}C_{r + 2} \\ {}^yC_r & {}^{y + 1}C_{r + 1} & {}^{y + 2}C_{r +
     2} \\ {}^zC_r & {}^{z + 1}C_{r + 1} & {}^{z + 2}C_{r + 2}\end{vmatrix}`

160. If :math:`\Delta_r = \begin{vmatrix}r & n + 1 & 1 \\ r^2 & 2n - 1 &
     \frac{2n + 1}{3} \\ r^3 & 3n + 2 & \frac{n(n + 1)}{2}\end{vmatrix},`

     show that :math:`\sum_{r = 1}^n \Delta_r = 0`

161. If :math:`\Delta_r = \begin{vmatrix}2^{r - 1} & 2.3^{r - 1} & 4.5^{r - 1}
     \\ x & y & z \\ 2^{n} - 1 & 3^n - 1 & 5^n - 1\end{vmatrix},`

     show that :math:`\sum_{r = 1}^n \Delta_r = 0`

162. Show without expanding that :math:`\begin{vmatrix} x^2 & (x - 1)^2 & (x -
     2)^2 \\ (x - 1)^2 & (x - 2)^2 & (x - 3)^2 \\ (x - 2)^2 & (x -
     3)^2 & (x - 4)^2\end{vmatrix}` is independent of :math:`x.`

163. Show without expanding that :math:`\begin{vmatrix}2 & 1 + i & 3 \\ 1 - i &
     0 & 2 + i \\ 3 & 2 - i & 1\end{vmatrix}` is purely real.

164. Show without expanding that :math:`\begin{vmatrix}x - 3 & 2x +1 & 2 \\
     3x + 2 & x + 2 & 1 \\ 5x + 1 & 5x + 4 & 5\end{vmatrix}` is independent of
     :math:`x.`

165. If :math:`a` and :math:`x` are real numbers and :math:`n` is a postive
     integer, then show without expanding that

     :math:`\begin{vmatrix}a^n - x & a^{n + 1} - x & a^{n + 2} - x \\ a^{n + 3}
     - x & a^{n + 4} - x & a^{n + 5} - x \\ a^{n + 6} - x & a^{n + 7} - x &
     a^{n + 8} - x\end{vmatrix} = 0`

166. Find :math:`\sum_{r = 2}^n (-2)^r \begin{vmatrix}{}^{n - 2}C_{r - 2} &
     {}^{n - 2}C_{r - 1} & {}^{n - 2}C_r \\ -3 & 1 & 1 \\ 2 & 1 &
     0\end{vmatrix}, n > 2`

167. If :math:`a,b,c` are non-zero real numbers, show without expanding that

     :math:`\begin{vmatrix}b^2c^2 & bc & b + c \\ c^2a^2 & ca & c + a \\ a^2b^2
     & ab & a + b\end{vmatrix} = 0`

168. Prove that :math:`\begin{vmatrix}b + c -a - d & bc - ad & bc(a + d) - ad(b
     + c) \\ c + a - b - d & ca - bd & ca(b + d) - bd(c + a) \\ a + b - c - d &
     ab - cd & ab(c + d) - cd(a + b)\end{vmatrix} = \\-2(b - c)(c - a)(a - b)(a -
     d)(b - d)(c - d)`

169. Prove that :math:`\begin{vmatrix}bc - a^2 & ca - b^2 & ba - c^2 \\ ca + ab
     - bc & bc + ab -ca & bc + ca - ab \\ (a + b)(a + c) & (b + c)(b + a) &
     (c + a)(c + b)\end{vmatrix} = \\3(b - c)(c - a)(a - b)(a + b + c)(ab +
     bc + ca)`

170. Prove that :math:`\begin{vmatrix}1 & (m + n - l - p)^2 & (m + n - l - p)^2
     \\ 1 & (n + l -m - p)^2 & (n + l -m - p)^4 \\ 1 & (l + m - n - p)^2 & (l +
     m - n - p)^4\end{vmatrix} = \\ 64(l - m)(l - n)(l - p)(m - n)(m - p)(n -
     p)`

171. If :math:`u, v, w` are differentiable functions of :math:`f` and suffixes
     denote the derivatives w.r.t. :math:`t`, prove that

     :math:`\frac{d}{dt}\begin{vmatrix}u_1 & v_1 & w_1 \\ u_2 & v_2 & w_2 \\
     u_3 & v_3 & w_3\end{vmatrix} = \begin{vmatrix}u_1 & v_1 & w_1 \\ u_2 & v_2
     & w_2 \\ u_4 & v_4 & w_4\end{vmatrix}`

172. If :math:`Y= sX` and :math:`Z = tX,` all the variables being
     differentiable functions of :math:`x,` prove that

     :math:`\begin{vmatrix}X & Y & Z \\ X_1 & Y_1 & Z_1 \\ X_2 & Y_2 &
     Z_2\end{vmatrix} = X^3\begin{vmatrix}s_1 & t_1 \\ s_2 & t_2\end{vmatrix}`
     where suffixes denote the derivative w.r.t. :math:`x.`

173. If :math:`f(x), g(x), h(x)` are polynomials in :math:`x` find the
     condition that

     :math:`\begin{vmatrix}f(x) & g(x) & h(x) \\ f(\alpha) & g(\alpha) &
     h(\alpha) \\ f(\beta) & g(\beta) & h(\beta)\end{vmatrix}`

     which a polynomial of degree :math:`3,` is exressible as :math:`a(x -
     \alpha)^2(x - \beta)`

174. Show that :math:`\begin{vmatrix}\sin(x + \alpha) & \cos(x + \alpha) & a +
     x\sin\alpha \\ \sin(x + \beta) & \cos(x + \beta) & b + x\sin\beta \\
     \sin(x + \gamma) & \cos(x + \gamma) & c +  x\sin\gamma\end{vmatrix}` is
     independent of :math:`x.`

175. If :math:`f(x) = \begin{vmatrix}2\cos^2x & \sin 2x & -\sin x \\ \sin 2x &
     2\sin^2 x & \cos x \\ \sin x & -\cos x & 0\end{vmatrix},` show that
     :math:`\int_{0}^{\frac{\pi}{2}} (f(x) + f'(x))dx = \pi`

176. Prove that :math:`\begin{vmatrix}a_1\alpha_1 + b_1\beta_1 & a_1\alpha_2 +
     b_1\beta_2 & a_1\alpha_3 + b_1\beta_3 \\ a_2\alpha_1 + b_2\beta_1 &
     a_2\alpha_2 + b_2\beta_2 & a_2\alpha_3 + b_2\beta_3 \\ a_3\alpha_1 +
     b_3\beta_1 & a_3\alpha_2 + b_3\beta_2 & a_3\alpha_3 +
     b_3\beta_3\end{vmatrix} = 0`

177. If :math:`l_r\vec{i}, m_r\vec{j}, n_r\vec{k}, r = 1,2,3` be three
     mutually perpendicular unit vectors, show that

     :math:`\begin{vmatrix}l_1 & l_2 & l_3 \\ m_1 & m_2 & m_3 \\ n_1 & n_2 &
     n_3\end{vmatrix} = \pm 1`

178. Let :math:`\Delta = \begin{vmatrix}a_1 & b_1 & c_1 \\ a_2 & b_2 & c_2 \\
     a_3 & b_3 & c_13\end{vmatrix}` and :math:`A_i, B_i, C_i` be the cofactors
     of :math:`a_i, b_i, c_i` respectively and :math:`\alpha_i, \beta_i,
     \gamma_i` be the cofactors of :math:`A_i, B_i, C_i` respectively, where
     :math:`i = 1,2,3,` show that

     :math:`\begin{vmatrix}A_1 & B_1 & C_1 \\ A_2 & B_2 & C_2 \\ A_3 & B_3 &
     C_3\end{vmatrix} \begin{vmatrix}\alpha_1 & \beta_1 & \gamma_1 \\ \alpha_2 &
     \beta_2 & \gamma_2 \\ \alpha_3 & \beta_3 & \gamma_3 \end{vmatrix} = \Delta^6`

179. Using determinants solve the equations:

     :math:`x + 2y + 3z = 6; 2x + 4y + z = 17; 3x + 2y + 9z = 2`

180. Solve the system of equations:

     :math:`ax + by + ca = d, a^2x + b^2y + c^2a = d^2; a^3x + b^3y + c^3a =
     d^3`

     Will the solution always exist and be unique?
 
181. Determine the coefficients :math:`a, b, c` of the quadratic function
     :math:`f(x)` where :math:`f(x) = ax^2 + bc + c` if :math:`f(1) = 0, f(2) =
     -2, f(3) = -6`

182. Determine the coefficients :math:`a, b, c` of the quadratic function
     :math:`f(x)` where :math:`f(x) = ax^2 + bc + c` if :math:`f(0) = 6, f(2) =
     11, f(-3) = 6` also find :math:`f(1).`

183. Solve

     :math:`\begin{array} (b + c)(y + z) - ax = b - c \\ (c + a)(z + x) -
     by = c - a \\ (a + b)(x + y) - cz = a - b\end{array}`

     where :math:`a + b + c \neq 0`

184. Examine the consistency of the system of equations

     :math:`7x - 7y + 5z = 3; 3x + y + 5z = 7; 2x + 3y + 5z = 5`

185. Find the value of :math:`k` for which the following system of equations are
     consistent

     :math:`x + y = 3; (1 + k)x + (2 + k)y = 8; x - (1 + k)y + (2 + k) = 0`

186. Find the value of :math:`k` for which the following system of equations are
     consistent

     :math:`(k + 1)^3x + (k + 2)^3y = (k + 1)^3; (k + 1)x + (k + 2)y = k + 3; x
     + y = 1`

187. Find the values of :math:`c` for which the equations

     :math:`2x + 3y = 3; (c + 2)x + (c + 4)y = c + 6; (c + 2)^2x + (c + 4)^2y =
     (c + 6)^2`

188. Find :math:`\lambda` for which the system of equations

     :math:`x + y - 2z = 0; 2x - 3y + z = 0; x - 5y + 4z = \lambda` are
     consistent and find the solutions for all such values of :math:`\lambda`

189. Find the value of :math:`\lambda` and :math:`\mu` for which the following
     system of equations

     :math:`x + y + z = 0; x + 2y + 3z = 14; 2x + 5y + \lambda z = \mu,
     \lambda, \mu \in R` has (i) unique solution (ii) infinite solutions.

190. If :math:`bc + qr = ca + rp = ab + pq = -1,` show that

     :math:`\begin{vmatrix}ap & a & p \\ bq & b & q \\ cr & c & r\end{vmatrix}
     = 0`

191. Find all values of :math:`k` for which the following system posses a
     non-trivial solution:

     :math:`x + ky + 3z = 0; kx + 2y + 2z = 0; 2x + 3y + 4z = 0`

192. If :math:`x = cy + bz; y = az + cx; z = bx + ay` where :math:`x,y,z` are
     not all zero. Prove that :math:`a^2 + b^2 + c^2 + 2abc = 1.`

     Further if at least one of :math:`a,b,c` is a proper fraction, prove that

     i. :math:`a^2 + b^2 + c^2 < 3`

     ii. :math:`abc > -1`

193. If :math:`a = \frac{x}{y - z}, b = \frac{y}{z - x}, c = \frac{z}{x - y}`
     where :math:`x,y,z` are not all zero, prove that :math:`1 + ab + bc + ca =
     0`

194. Consider the system of linear equations, in :math:`x,y,z`:

     :math:`\begin{array}((\sin 3\theta)x - y + z = 0\\ (\cos 2\theta)x + 4y +
     3z = 0 \\ 2x + 7y + 7z = 0\end{array}`

     Find the value of :math:`\theta` for which this system has non-trivial
     solution.

195. If :math:`a,b,c` are in G.P. with common ration :math:`r_1`and
     :math:`\alpha, \beta, \gamma` are in G.P. with common ratio :math:`r_2,`
     then find the conditions that :math:`r_1`and :math:`r_2` must satisfy in
     order that the equations

     :math:`ax + \alpha y + z = 0; bx + \beta y + z = 0; cx + \gamma y + z = 0`

     have only trivial solutions.
