Logarithm Solutions Part 1
**************************
1. :math:`\log_{\sqrt{8}}x = \frac{10}{3} \Rightarrow \log_2^{\frac{3}{2}} x = \frac{10}{3}`

   :math:`\Rightarrow \frac{2}{3}\log_2 x = \frac{10}{3} \Rightarrow \log_2 x = 5`

   :math:`\Rightarrow x = 25`

2. L.H.S. :math:`= \log_b a.\log_c b.\log_a c = \frac{\log a}{\log b}\frac{\log
   b}{\log c}\frac{\log c}{\log a} = 1`

3. L.H.S. :math:`= \log_3 \log_2 \log_{\sqrt{5}} (625) = \log_3 \log_2
   \log_{\sqrt{5}} 5^4`

   :math:`= \log_3 \log_2 8 = \log_3 \log_2 2^3 = \log_3 3 = 1`

4. Given, :math:`a^2 + b^2 = 23ab \Rightarrow (a + b)^2 = 25ab`

   :math:`\Rightarrow \left(\frac{a + b}{5}\right) = \sqrt{ab}`

   Taking log on both sides, we get

   :math:`\log \frac{a + b}{5} = \frac{1}{2}(\log a + \log b)`

5. L.H.S. :math:`= 7\log \frac{16}{15} + 5\log \frac{25}{24} + 3\log
   \frac{81}{80}`

   :math:`= 7[\log 2^4 - \log(3.5)] + 5[\log 5^2 - \log 2.2.2.3] + 3[\log 3^4 -
   \log 2^4.5]`

   :math:`= 7[4\log2 - \log 3 - \log 5] + 5[2\log 5 - 3\log 2 -\log 3] + 3[4\log
   3 - 4\log 2 -\log 5]`

   :math:`= \log 2 =` R.H.S.

6. L.H.S. :math:`=\log\tan 1^{\circ} + \log\tan 2^{\circ} + \ldots +
   \log \tan 89^{\circ}`

   :math:`= \log(\tan 1^{\circ}.\tan 89^{\circ}).\log(\tan 2^{\circ}.\tan
   88^{\circ}) \ldots \log \tan 45^{\circ}`

   :math:`= \log(\tan 1^{\circ}.\cot 1^{\circ}).\log(\tan 2^{\circ}.\cot
   2^{\circ}) \ldots \log \tan 45^{\circ}`

   :math:`= \log 1.\log 1\ldots \log 1 = 0`

7. :math:`\log_9 \tan \frac{\pi}{6} = \log_9 \frac{1}{\sqrt{3}} = \log_3^2
   3^{-\frac{1}{2}}`

   :math:`= \frac{1}{2}\log_3 3^{-\frac{1}{2}} = \frac{1}{2}.-\frac{1}{2} =
   -\frac{1}{4}`

8. :math:`\frac{\log_{a^2}b}{\log_{\sqrt{a}}(b)^2} = \frac{\frac{1}{2}\log_a
   b}{2.2\log_a b}`

   :math:`= \frac{\log_a b}{8\log_a b} = \frac{1}{8}`

9. :math:`\log_{\sqrt{5}}.008 = 2\log_5 \frac{8}{1000} = 2[\log_5 8 - \log_5
   1000]`

   :math:`= 2[\log_5 8 - \log_5 8 - \log 125] = -6`

10. :math:`\log_{2\sqrt{3}}144 = \log_{2\sqrt{3}}12^2 =
    \log_{2\sqrt{3}}(2\sqrt{3})^4 = 4`

11. L.H.S. :math:`=\log_3 \log_2 \log_{\sqrt{3}} 81 = \log_3 \log_2
    \log_{\sqrt{3}}(\sqrt{3})^8`

    :math:`= \log_3 \log_2 8 = \log_3 \log_2 2^3 = \log_3 3 = 1`

12. L.H.S. :math:`= \log_a x \log_b y = \frac{\log x}{\log a}\frac{\log y}{\log
    b}`

    :math:`= \frac{\log x}{\log b}\frac{\log y}{\log a} = \log_b x \log_a y =`
    R.H.S.

13. L.H.S. :math:`= \log_2 \log_2 \log_2 16 = \log_2 \log_2 \log_2 2^4 = \log_2
    \log_2 4 = \log_2 \log_2 2^2 = \log_2 2 = 1 =` R.H.S.

14. R.H.S. :math:`= \log_b x\log_c b \ldots \log_n m \log_a n = \frac{\log
    x}{\log b}\frac{\log b}{\log c}\ldots \frac{\log m}{\log n}\frac{\log
    n}{\log a}`

    :math:`= \frac{\log x}{\log a} = \log_a x =` L.H.S.

15. R.H.S. :math:`= 10^x\log_{10}a = z` (say)

    Taking log of both sides with base :math:`10`

    :math:`\log_{10} z =x\log_{10}a = \log_{10}a^x \Rightarrow z = a^x =`
    L.H.S.

16. Given, :math:`a^2 + b^2 = 7ab \Rightarrow a^2 + b^2 + 2ab = 9ab`

    :math:`\Rightarrow \left(\frac{a + b}{3}\right)^2 = ab`

    Taking log of both sides

    :math:`\Rightarrow 2\log \left(\frac{a + b}{3}\right) = \log ab = \log a +
    \log b`

    :math:`\Rightarrow \log \left\{\frac{1}{3}(a + b)\right\} =
    \frac{1}{2}(\log a + \log b)`

17. L.H.S. :math:`= \frac{\log a(\log_b a)}{\log b(\log_a b)} = \frac{\log a
    \frac{\log a}{\log b}}{\log b \frac{\log a}{\log b}}`

    :math:`= \frac{\log a\log a - \log a \log b}{\log b \log b - \log b \log
    a}`

    :math:`\frac{\log a(\log a - \log b)}{\log b(\log b - \log a)} = - \log_b a
    =` R.H.S.

18. L.H.S. :math:`= \log(1 + 2 + 3) = \log 6 = \log 2.3 = 0 + \log 2 + \log 3`

    :math:`= \log 1 + \log 2 + \log 3[\because \log 1 = 0]`

19. L.H.S. :math:`= 2\log(1 + 2 + 4 + 7 + 14) = 2\log 28 = \log 28^2 = \log
    784`

    :math:`= \log 1*2*4*7*14 = \log 1 + \log 2 + \log 4 + \log 7 + \log 14`

20. L.H.S. :math:`= \log 2 + 16\log \frac{16}{15} + 12\log \frac{25}{24} +
    7\log \frac{81}{80} = 1`

    :math:`= \log 2 + 16[\log 16 - \log 15] + 12[\log 25 - \log 24] + 7[\log
    81 - \log 80]`

    :math:`= \log 2 + 16[\log 2^4 - \log 3*5] + 12[\log 5^2 - \log 2^3*3] +
    7[\log 3^4 - \log 2^4*5]`

    :math:`= \log 2 + 16[4\log 2 - \log 3 -\log 5] + 12[2\log 5 - 3\log 2 -\log
    3] + 7[4\log 3 - 4\log 2 -\log 5]`

    :math:`= \log 2[1 + 64 - 36 - 28] + \log 3[28 - 16 - 12] + \log 5[24 - 7 -
    16]`

    :math:`= \log 2 + \log 5 = \log 10 = 1` [default base is :math:`10` for
    common logarithms]

21. Given, :math:`\frac{\log_9 11}{\log_5 13} \div \frac{\log_3
    11}{\log_{\sqrt{5}} 13}`

    :math:`= \frac{\log_{3^2} 11}{\log_5 13}\frac{\log_{5^{\frac{1}{2}}}
    13}{\log_3 11}`

    :math:`= \frac{\frac{1}{2}\log_3 11}{\log_5 13}\frac{2\log 13}{\log_3 11} =
    1`

22. Given, :math:`3^{\sqrt{\log_3 2}} - 2^{\sqrt{\log_2 3}}`

    Taking log with base :math:`10,` we get

    :math:`=\sqrt{\log_3 2}\log 3 - \sqrt{\log_2 3}\log 2`

    :math:`= \sqrt{\frac{\log 2}{\log 3}(\log 3)^2} - \sqrt{\frac{\log 3}{\log
    2}(\log 2)^2}`

    :math:`= \sqrt{\log 2\log 3} - \sqrt{\log 3\log 2} = 0`

23. Given :math:`\log_{10} 343 = 2.5353 \Rightarrow \log_{10} 7^3 = 2.5353
    \Rightarrow \log_{10} 7 = .8451`

    For, :math:`7^n > 10^5 \Rightarrow n\log_{10}7 = 5\Rightarrow n =
    \frac{5}{.8451}`

    Thus, least such integer is :math:`6`

24. Since :math:`a, b, c` are in G.P., we can write :math:`b^2 = ac`

    Taking log of both sides

    :math:`2\log b = \log a + \log c`

    Thus, :math:`\log a, \log b, \log c` are in A.P.

    i.e. :math:`\frac{1}{\log a}, \frac{1}{\log b}, \frac{1}{\log c}` are in
    H.P.

    Multiplying each term with :math:`\log x`

    i.e. :math:`\frac{\log x}{\log a}, \frac{\log x}{\log b}, \frac{\log
    x}{\log c}` are in H.P.

    i.e. :math:`\log_a x, \log_b x, \log_c x` are in H.P.

25. L.H.S. :math:`= \log \sin 8x = \log 2\sin 4x \cos 4x`

    :math:`= \log 2 + \log \sin 4x + \log \cos 4x`

    :math:`= \log 2 + \log 2\sin 2x\cos 2x + \log \cos 4x`

    :math:`= 2\log 2 + \log \sin 2x + \log \cos 2x + \log \cos 4x`

    :math:`= 2\log 2 + \log 2\sin x\cos x + \log \cos 2x + \log \cos 4x`

    :math:`= 3\log 2 + \log \sin x + \log \cos x + \log \cos 2x + \log \cos 4x`

26. We have to prove :math:`xyz + 1 = 2yz`

    Dividing both sides by :math:`yz,` we get

    :math:`x + \frac{1}{yz} = 2`

    L.H.S. :math:`= \log_{2a}a + \frac{1}{\log_{3a}2a\log_{4a}3a}`

    :math:`= \frac{\log a}{\log 2a} + \frac{\log 3a}{\log 2a}\frac{\log
    4a}{\log 3a}`

    :math:`=\frac{\log a}{\log 2a} + \frac{\log 4a}{\log 2a}`

    :math:`= \frac{\log a + \log 4a}{\log 2a} = \frac{\log (2a)^2}{\log 2a} =
    2`

27. We have to prove that :math:`\log_{c + b} a + \log_{c - b} a = 2\log_{c +
    b}a\log_{c -b}a`

    Dividing both sides by :math:`\log_{c + b}a\log_{c -b}a,` we get

    :math:`\frac{1}{\log_{c - b}a} + \frac{1}{\log_{c + b}a} = 2`

    :math:`\log_a(c - b) + \log_a(c + b) = 2`

    :math:`\log_a(c^2 - b^2) = 2`

    :math:`c^2 - b^2 = a^2`

    :math:`c^2 = a^2 + b^2` which is true because :math:`c` is hypotenuse and
    :math:`a` and :math:`b` are sided of a right angle triangle.

28. We have to prove that, :math:`x^xy^yz^z = 1`

    Taking log of both sides

    :math:`x\log x + y\log y + z\log z = 0`

    Let :math:`\frac{\log x}{y - z} = \frac{\log y}{z - x} = \frac{\log z}{x -
    y} = k`

    :math:`\log x = k(y - z), \log y = k(z - x), \log z = k(x - y)`

    :math:`x\log x + y\log y + z\log z = k(xy - zx + yz - xy + zx - yz) = 0`

29. Given, :math:`\frac{yz\log(yz)}{y + z} = \frac{zx\log(zx)}{z + x} =
    \frac{xy\log(xy)}{x + y}`

    Dividing each term by :math:`xyz,` we get

    :math:`\frac{\log(yz)}{x(y + z)} = \frac{\log(zx)}{y(z + x)} =
    \frac{\log(xy)}{z(x + y)}`

    :math:`\frac{\log y + \log z}{xy + zx} = \frac{\log z + \log x}{yz + xy} =
    \frac{\log x + \log y}{zx + yz} = k` (let)

    :math:`\log y + \log z = k(xy + zx), \log z + \log x = k(yz + zx), \log x +
    \log y = k(zx + yz)`

    Adding all these, we get

    :math:`2(\log x + \log y + \log z) = 2k(xy + yz + xz)`

    :math:`(\log x + \log y + \log z) = k(xy + yz + xz)`

    :math:`\therefore \log x = kyz \Rightarrow x\log x = kxyz`

    Similarly :math:`y\log y = kxyz` and :math:`z\log z = kxyz`

    :math:`\therefore x\log x = y\log y = z\log z = kxyz`

    :math:`\Rightarrow x^x = y^y = z^z`

30. We have to prove that :math:`(yz)^{\log y - \log z}(zx)^{\log z - \log
    x}(xy)^{\log x -\log y} = 1`

    Taking log of both sides

    :math:`(\log y - \log z)(\log y + \log z) + (\log z - \log x)(\log z - \log
    x) + (\log x - \log y)(\log x + \log y) = 0`

    :math:`(\log y)^2 - (\log z)^2 + (\log z)^2 - (\log x)^2 + (\log x)^2 -
    (\log y)^2 = 0`

    :math:`0 = 0`

31. We have to prove that :math:`\frac{1}{\log_2 N} + \frac{1}{\log_3 N} +
    \ldots + \frac{1}{\log_{1988} N} = \frac{1}{\log_{1988!} N}`

    L.H.S. :math:`= \log_N 2 + \log_N 3 + \ldots + \log_N 1988`

    :math:`= \log_N (2.3.4\ldots 1988)`

    :math:`= \log_N 1988! = \frac{1}{\log_{1988!}N}`

32. L.H.S. :math:`= \log(1 + x) + \log(1 + x^2) + \log(1 + x^4) \ldots` to
    :math:`\infty`

    :math:`\log (1 + x + x^3 + x^4 + \ldots)` to :math:`\infty`

    :math:`= \log \frac{1}{1 - x}~[\because |x| < 1]`

    :math:`= -\log(1 - x)`

33. Let :math:`S_n = \frac{1}{\log_2 a} + \frac{1}{\log_4 a} + \ldots` upto
    :math:`n` terms`

    :math:`S_n = \log_a 2 + \log_a 4 + \log_a 8 + \ldots` upto :math:`n` terms

    :math:`S_n = (1 + 2 + 3 + \ldots + n)\log_a 2`

    :math:`= \frac{n(n + 1)}{2}\log_a 2`

34. L.H.S. :math:`= \frac{1}{x + 1} + \frac{1}{y + 1} + \frac{1}{z + 1}`

    :math:`= \frac{1}{\log_4 10 + \log_{4} 4} + \frac{1}{\log_{2}20 + \log_2 2}
    + \frac{1}{\log_5 8 + \log_5 5}`

    :math:`= \frac{1}{\log_4 40} + \frac{1}{\log_2 40} + \frac{1}{\log_4 40}`

    :math:`= \log_{40} 4 + \log_{40} 2 + \log_{40} 5 = \log_{40} 40 = 1`

35. We have to prove that :math:`\frac{1}{x + 1} + \frac{1}{y + 1} +
    \frac{1}{z + 1} = 1`

    L.H.S. :math:`= \frac{1}{=log_a{bc} + 1} + \frac{1}{\log_b(ca) + 1} +
    \frac{1}{\log_c(ab) + 1}`

    :math:`= \frac{1}{=log_a{bc} + \log_a a} + \frac{1}{\log_b(ca) + \log_b
    b} + \frac{1}{\log_c(ab) + \log_c c}`

    :math:`= \frac{1}{\log_a(abc)} + \frac{1}{\log_b(abc)} +
    \frac{1}{\log_c(abc)}`

    :math:`= \log_{abc}a + \log_{abc}b + \log_{abc}c = \log{abc}abc = 1`

36. We have to prove that :math:`\frac{1}{1 + \log_b a + \log_b c} +
    \frac{1}{1 + \log_c a + \log_c b} + \frac{1}{1 + \log_a b + \log_a c} = 1`

    L.H.S. :math:`= \frac{1}{\log_b b + \log_b a + \log_b c} +
    \frac{1}{\log_c c + \log_c a + \log_c b} + \frac{1}{\log_a a + \log_a b +
    \log_a c}`

    :math:`= \frac{1}{\log_b abc} + \frac{1}{\log_c abc} + \frac{1}{\log_a
    abc}`

    Like previus exercise above expression evaluates to :math:`1`

37. We have to prove that :math:`x^{\log y - \log z}y^{\log z - \log x}z^{\log
    x - \log y} = 1`

    Taking log of both sides

    :math:`(\log y - \log z)\log x + (\log z - \log x)\log y + (\log x - \log
    y)\log z = 0`

    :math:`\log y\log x - \log z\log x + \log z\log y - \log x\log y + \log
    x\log z - \log y\log z = 0`

    :math:`0 = 0`

38. We have to prove that :math:`a^xb^yc^z = 1`

    :math:`x\log a + y\log b + z\log c = 0`

    Let :math:`\frac{\log a}{y - z} = \frac{\log b}{z - x} = \frac{\log
    c}{x - y} = k`

    :math:`x\log a = k(xy - zx), y\log b = k(yz - xy), z\log c = k(zx - yz)`

    Adding all these

    :math:`x\log a + y\log b + z\log c = k(xy -zx + yz - xy + zx - yz) = 0`

39. Let :math:`\frac{x(y + z - x)}{\log x} = \frac{y(z + x - y)}{\log y} =
    \frac{z(x + y - z)}{\log z} = \frac{1}{k}`

    :math:`\log x = kx(y + z - x), \log y = ky(z + x - y), \log z = kz(x + y -
    z)`

    Let :math:`y^zz^y = z^xx^z = x^yy^x = c`

    Taking log :math:`z\log y + y\log z = x\log z + z\log x = y\log x + x\log y
    = log c`

    :math:`\Rightarrow zky(z + x - y) + ykz(x + y - z) = xkz(x + y - z) +
    zkx(y + z - x)\\ = ykx(y + z - x) + xky(x + z - y)`

    :math:`\Rightarrow yz^2 + xyz - y^2z + xyz + y^2z - z^2y = x^2z + xyz
    -xz^2 + xyz + xz^2 - x^2z\\ = xy^2 + xyz - x^2y + x^2y + xyz - xy^2`

    :math:`\Rightarrow 2xyz = 2xyz = 2xyz`

40. Let :math:`\frac{\log a}{b - c} = \frac{\log b}{c - a} = \frac{\log c}{a -
    b} = k`

    :math:`\log a = k(b - c), \log b = k(c - a), \log c = k(a - b)`

    We have to prove that :math:`a^{b + c}b^{c + a}c^{a + b} = 1`

    Taking log of both sides, we get

    :math:`(b + c)\log a + (c + a)\log b + (a + b)\log c = 0`

    Substituting the values, we get

    :math:`k(b^2 - c^2) + k(c^2 - a^2) + k(a^2 - b^2) = 0`

41. Let :math:`\frac{\log x}{q - r} = \frac{\log y}{r - p} = \frac{\log z}{p -
    q} = k`

    :math:`\log x = k(q - r), \log y = k(r - p), \log z = k(p - q)`

    We have to prove that :math:`x^{q + r}y^{p + r}z^{p + q} = x^py^qz^r`

    Taking log of both sides, we get

    :math:`(q + r)\log x + (p + r)\log y + (p + q)\log z = p\log x + q\log y +
    r\log z`

    Substituting the value of :math:`\log x, \log y, \log z`

    :math:`k(q^2 - r^2) + k(r^2 - p^2) + k(p^2 - q^2) = k(pq - pr + qr - pq +
    pq - qa)`

    :math:`0 = 0`

42. Given :math:`y = a^{\frac{1}{1 - \log_a x}}` and :math:`z = a^{\frac{1}{1 -
    \log_a y}}`

    :math:`z = a^{\frac{1}{1 - \log_a (a^{\frac{1}{1 - \log_a x}})}}`

    :math:`z = a^{\frac{1}{1 - \frac{1}{1 - \log_a x}}}`

    Taking log of both sides with base :math:`a,` we get

    :math:`\log_a z = \frac{1}{1- \frac{1}{1 - \log_a x}}`

    :math:`\log_a z = \frac{1- \log_a x}{-\log_a x} = 1 - \frac{1}{\log_a x}`

    :math:`x = a^{\frac{1}{1 - \log_a z}}`

43. Given :math:`f(y) = e^{f(z)}` and :math:`z= e^{f(x)},` where :math:`f(x) =
    \frac{1}{1 - \log_e x}`

    :math:`f(y) = e^{\frac{1}{1 - \log_e z}}`

    :math:`z = e^{\frac{1}{1- \log_e x}}`

    :math:`f(y) = e^{\frac{1}{1 - \log_e z}} = e^{\frac{1}{1 - \log_e
    e^{\frac{1}{1 - \log_e x}}}}`

    :math:`f(y) = e^{\frac{1}{1 - \frac{1}{1 -\log_e x}}}`

    Following like exercise above

    :math:`x = e^{f(y)}`

44. L.H.S. :math:`= \frac{1}{\log_2 n} + \frac{1}{\log_3 n} + \frac{1}{\log_4
    n} + \ldots + \frac{1}{\log_{43} n}`

    :math:`= \log_n 2 + \log_n 3 + \log_n 4 + \ldots + \log_n 43`

    :math:`=\log_n(2.3.4\ldots 43) = \log_n 43! = \frac{1}{\log_{43!}n} =`
    R.H.S.

45. L.H.S. :math:`= 2(\log a + \log a^2 + \log a^3 + \ldots + \log a^n)`

    :math:`=2\log a(1 + 2 + 3 + \ldots + n) = 2\log a \frac{n(n + 1)}{2}`

    :math:`= n(n + 1)\log a`

46. We will make use of the fact that positive characteristics of :math:`n` of
    a logarithm means there are :math:`n + 1` digits in the number.

    Let :math:`\log y = 12\log 12 = 12\log 2.2.3`

    :math:`= 12[2*.301 + .477] = 12.96`

    Thus, number of digits is :math:`13`.

47. Here we can use the result that number of positive integers having base
    :math:`b` and characteristics :math:`n` is :math:`b^{n + 1}- b^n`

    Thus, number of integers with base :math:`3` and characteristics :math:`2`
    is :math:`3^3 - 3^2 = 18.`

48. L.H.S. :math:`= \log_a x\log_b y`

    :math:`= \frac{\log x}{\log a}\frac{\log y}{\log b}`

    :math:`= \frac{\log x}{\log b}\frac{\log y}{\log a}`

    :math:`\log_bx\log_ay =` R.H.S.

49. Given, :math:`a, b, c` are in G.P.

    :math:`\frac{b}{a} = \frac{c}{b}`

    :math:`\log_x \frac{b}{a} = \log_x \frac{c}{b}`

    :math:`\log_x b - \log_x a = \log_x c - \log_x b`

    :math:`\log_xa, \log_xb, \log_xc` are in A.P.

    :math:`\log_a x, \log_b x, \log_c x` are in H.P.

50. Let :math:`y = (0.0504)^{10}`

    :math:`\log_{10}y = 10\log_{10}(.0504) = 10\log_{10}(504*10^{-4})`

    :math:`= -10\log_{10}[-4 + \log(2^3.3^2.7)]`

    :math:`= -12.98`

    Thus, chraracteristics is :math:`-13`

    Therefore, number of zeroes after decimal and first significant digit :math:`= 12`
