Logarithm Solutions Part 3
**************************
101. Given, :math:`\log_2(x^2 - 24) > \log_2 5x`

     Since base is greater than one, we can say that

     :math:`x^2 - 24 > 5x`

     :math:`(x - 8)(x + 3) > 0`

     :math:`-3 > x, x > 8`

     But :math:`x^2 - 24 > 0` and also :math:`x > 0` for logarithm function to
     be defined.

     :math:`\therefore` the solutions is :math:`x > 8`

102. We have to prove that :math:`\frac{1}{\log_3\pi} + \frac{1}{\log_4\pi} >
     2`

     :math:`\Rightarrow \log_{\pi} 3 + \log_{\pi} 4 > 2`

     :math:`\Rightarrow \log_{\pi} 12 > 2`

     :math:`\Rightarrow 12 > \pi^2` which is true.

103. Given :math:`(0.01)^{\frac{1}{3}}` and :math:`(0.001)^{\frac{1}{5}}`

     Taking logarithmg of both with base :math:`10`

     :math:`\frac{1}{3}\log_{10} 0.01` and :math:`\frac{1}{5}\log_{10}0.001`

     :math:`\frac{-2}{3}` and :math:`\frac{-3}{5}`

     Since :math:`\frac{-3}{5}` is greater, :math:`\therefore
     (0.001)^{\frac{1}{5}}` is greater.

104. :math:`\log_311>\log_39=\log_3(3^2)=2` and
     :math:`\log_23<\log_24=\log_2(2^2)=2`

     Thus, :math:`\log_311` is greater.

185. :math:`\log_3(x^2 + 10) > \log_3 7x`

     :math:`\Rightarrow x^2 + 10 > 7x\Rightarrow x < 2, x > 5`

     However, :math:`x^2 + 10 > 0` and :math:`x > 0`

     Thus, intervals are :math:`0 < x < 2` and :math:`x > 5`

106. We have, :math:`x^{\log_{10} x} > 10`

     :math:`\Rightarrow\log_{10}x \log_{10} x  > 1`

     :math:`\log_{10}x > \pm 1`

     Thus the range for values of :math:`x` would be :math:`(0, 0.1)\cup(10,
     \infty]`

107. We have :math:`\log_2 x\log_{2x} 2\log_2 4x > 1`

     :math:`\frac{1}{\log_x 2}\left[\frac{1}{\log_2 2x}\log_2 2^2 x\right] > 1`

     :math:`\frac{1}{\log_x 2}\left[\frac{1}{1 + \log x}\right]\left[2 +
     \frac{1}{\log_x 2}\right] > 1`

     Let :math:`z = \log_x 2` then the above inequality becomes

     :math:`\frac{1}{z}\left[\frac{1}{1 + z}\right]\left[2 + \frac{1}{t}\right]
     > 1`

     Solving this inequality and applying rules for base of a logarithm we will
     have following range for :math:`x, \left(2^{-\sqrt{2}},
     \frac{1}{2}\right)\cup\left(1, 2^{\sqrt{2}}\right)`

108. Given, :math:`\log_2 x\log_3 2x + \log_3 x\log_2 4x > 0`

     Exchaning base, we have :math:`\log_3 x\log_2 2x + \log_3 x\log_2 4x > 0`

     :math:`\log_3 x(\log_2 2 + \log_2 x + \log_2 4 + \log_2 x) > 0`

     :math:`\log_3 x(3 + 2\log_2 x) > 0`

     For, :math:`\log_3 x > 0, x > 1`

     and for, :math:`3 + \log_2 x^2 > 0`

     :math:`\log_2 x^2 > -3`

     Also, for :math:`\log_3 x < 0, 0 < x < 1` and for

     :math:`3 + \log_2 x^2 < 0`

     :math:`\log_2 x^2 < -3`

109. :math:`\log_{12}60 = \frac{\log_260}{\log_212} = \frac{\log_2(2^2 \times
     3\times 5)}{\log_2 (2^2\times 3)}`

     :math:`= \frac{2 + \log_23 + \log_25}{2 + \log_23}`

     Let :math:`\log_23 = x` and :math:`\log_25 = y`

     :math:`\log_{12}60 = \frac{2 + x + y}{2 + x}`

     Given, :math:`a = \log_630 = \frac{\log_230}{\log 26} =
     \frac{\log_2(2\times 3\times 5)}{\log_2(2\times 3)}`

     :math:`= \frac{1 + \log_23 + \log_25}{1 + \log_23} = \frac{1 + x + y}{1 +
     x}`

     Also given that, :math:`b= \log_{15}24 = \frac{\log_224}{\log_215} =
     \frac{\log_2(2^3\times 3)}{\log_2 (3\times 5)}`

     :math:`= \frac{3 + \log_23}{\log_23 + \log_25} = \frac{3 + x}{x + y}`

     From these values of :math:`a` and :math:`b` in terms of :math:`x` and
     :math:`y,` we get

     :math:`x = \frac{b + 3 - ab}{ab - 3}, y = \frac{2a - b - 2 + ab}{ab - 1}`

     Substituting these value of :math:`x` and :math:`y` for
     :math:`\log_{12}60,` we get

     :math:`\log_{12}60 = \frac{2ab + 2a - 1}{ab + b + 1}`

110. Since :math:`\log_ax, \log_bx` and :math:`\log_cx` are in A.P.

     :math:`2\log_bx = \log_ax + \log_cx`

     :math:`\frac{2}{\log_xb} = \frac{1}{\log_xa} + \frac{1}{\log_xc}`

     :math:`\frac{2}{\log_xb} = \frac{\log_xa + \log_xc}{\log_xa\log_xc}`

     :math:`\frac{2}{\log_xb} = \frac{\log_xac}{\log_xa\log_xc}`

     :math:`2\log_xc = \log_xac\frac{\log_xb}{\log_xa}`

     :math:`\log_xc^2 = \log_xac\log_ab`

     :math:`c^2 = ac^{\log_ab}`

111. We have to use following rules:

     If :math:`b > 0, N > 0` or  :math:`b < 0, N< 0,` then :math:`\log_bN > 0`

     else if :math:`b > 0, N < 0` or :math:`b < 0, N > 0,` then :math:`\log_bN
     < 0`

     :math:`a = \log_{\frac{1}{2}}(\sqrt{0.125}) > 0` because both base and
     number are less than :math:`0`

     :math:`b = \log_3\left(\frac{1}{\sqrt{24} - \sqrt{17}}\right)`

     :math:`= \log_3\left(\frac{\sqrt{24} + \sqrt{17}}{(\sqrt{24} -
     \sqrt{17)(\sqrt{14} + \sqrt{17})}}\right)`

     :math:`= \log_3 \left(\frac{\sqrt{24} + \sqrt{17}}{7}\right) > 0` because
     both base and number are greater than :math:`0`

112. Given, :math:`e^{\frac{-\pi}{2}} < \theta < \frac{\pi}{2}`

     Taking log natural of both sides

     :math:`\log_ee^{-\frac{\pi}{2}} < \log_e\theta < \log_e\frac{\pi}{2}`

     :math:`\Rightarrow -\frac{\pi}{2} < \log_e\theta < 1<
     \frac{\pi}{2}\left[\because \log_e \frac{\pi}{2} <  \log_ee\right]`

     :math:`\Rightarrow -\frac{\pi}{2} < \log_e\theta < \frac{\pi}{2}`

     :math:`\Rightarrow \cos(\log_e\theta) > 0`

     Also, :math:`e^{\frac{-\pi}{2}} < \theta < \frac{\pi}{2}`

     :math:`\Rightarrow 0 < \theta < \frac{\pi}{2}\left[\because
     e^{-\frac{\pi}{2}} > 0\right]`

     :math:`\Rightarrow 0 < \cos\theta < 1`

     :math:`\Rightarrow \log_e \cos\theta < 0`

     :math:`\therefore \cos(\log_e\theta > \log_e(\cos\theta))`

113. Given, :math:`\log_2 x + \log_2 y \geq 6`

     :math:`\log_2xy \geq 6,\Rightarrow xy \geq 64`

     This means :math:`x` and :math:`y` are positive as negative vlaues will
     not be valid for logarithm function.

     A.M. :math:`\geq` G.M.

     :math:`\frac{x + y}{2} \geq \sqrt{xy}`

     :math:`x + y \geq 16`

114. Given, :math:`\log_b a \log_c a - \log_a a + \log_a b\log_c b - \log_b b +
     \log_a c \log _b c - \log_c c = 0`

     :math:`\frac{(\log_a)^2}{\log b \log c} - 1 + \frac{(\log b)^2}{\log a
     \log c} - 1 + \frac{(\log c)^2}{\log a\log b} - 1 = 0`

     Let :math:`\log a = x, \log b = y, \log c = z,` then we have

     :math:`\frac{x^2}{yz} + \frac{y^2}{zx} + \frac{z^2}{xy} - 3 = 0`

     :math:`\frac{x^3 + y^3 + z^3 - 2xyz}{xyz} = 0`

     :math:`(x + y + z)(x^2 + y^2 + z^2 - xy - yz - xz) = 0`

     :math:`(x + y + z)\frac{1}{2}[(x - y)^2 + (y - z)^2 + (z - x)^2] = 0`

     :math:`\because x, y , z` are different the term inside brackets will be
     always positive. Thus,

     :math:`x + y + z = 0,` now substituting the original values we get

     :math:`\log abc = 0, \Rightarrow abc = 1`

115. Given, :math:`y = 10^{\frac{1}{1 - \log x}}`

     Taking logarithm of both sides we get

     :math:`\log y = \frac{1}{1 - \log x}`

     Also, :math:`z = 10^{\frac{1}{1 - \log y}}`

     :math:`\log z = \frac{1}{1 - \log y}`

     :math:`\Rightarrow log y = 1 - \frac{1}{\log z}`

     Equating the values for :math:`\log y,` we get

     :math:`\frac{1}{1 - \log x} = 1 - \frac{1}{\log z}`

     :math:`\log x = \frac{1}{1 - \log z}`

     :math:`x = 10^{\frac{1}{1 - \log z}}`

116. Since :math:`n` is natural numbers and
     :math:`p_1, p_2, p_3, \ldots, p_k` are distinct primes, therefore
     :math:`a_1, a_2, \ldots, a_k` are also natural numbers.

     Now, :math:`n = p_1^{a_1}p_2^{a_2}p_3^{a_3} \ldots p_k^{a_k}`

     :math:`\log n = a_1\log p_1 + a_2\log p_2 + \ldots + a_k \log p_k`

     :math:`\log n \geq \log 2 + \log 2 + \ldots + \log 2` [since bases are
     primes so minimum value if :math:`2` and powers are natural numbers so
     they are greater than 1]

     :math:`\log n \geq k\log 2`

117. Let :math:`d` be the common difference of this A.P. then we can write

     :math:`3\log_y x = 3 +d\Rightarrow \log_yx^3 = 3 + d\Rightarrow x^3 =
     y^{(3 + d)}`

     :math:`3\log_z y = 3 + 2d\Rightarrow y^3 = z^{(3 + 2d)}`

     :math:`7\log_x z = 3 + 3d\Rightarrow z^7 = x^{(3 + 3d)}`

     :math:`y^3 = z^{(3 + 2d)}\Rightarrow y = z^{\frac{3 + 2d}{3}}`

     :math:`x^3 = y^{(3 + d)}\Rightarrow x = y^{\frac{3 + d}{3}} =
     z^{\frac{(3 + d)(3 + 2d)}{9}}`

     :math:`z^7 = x^{(3 + 3d)}\Rightarrow x = z^\frac{7}{3 + 3d}`

     Thus, :math:`\frac{(3 + d)(3 + 2d)}{9} = \frac{7}{3 + 3d}`

     :math:`\Rightarrow d = \frac{1}{2}`

     Thus, :math:`x^{18} = y^{21} = z^{28}`

118. We have :math:`\log_418 = \log_{2^2}(2\times 3^2) = \frac{1}{2} + \log_23`

     Thus, it will be enough to prove that :math:`\log_23` is an irrational
     number.

     Let :math:`\log_23 = \frac{p}{q}` where :math:`p, q \in I`

     :math:`2^{\frac{p}{q}} = 3\Rightarrow 2^p = 3^q`

     However, :math:`2^p` is an even number while :math:`3^q` is an odd number,
     and hence the equality will never be achieved. Therefore :math:`\log_23`
     is an irrational number.

119. :math:`\because x, y, z` are in G.P.

     :math:`\frac{y}{x} = \frac{z}{y}`

     :math:`\ln \frac{y}{x} = \ln \frac{z}{y}`

     :math:`\ln y - \ln x = \ln z - \ln x`

     :math:`\ln x, \ln y, \ln z` are in A.P.

     :math:`1 + \ln x, 1 + \ln y, 1 + \ln z` are in A.P.

     :math:`\frac{1}{1 + \ln x}, \frac{1}{1 + \ln y}, \frac{1}{1 + \ln z}` are
     in H.P.

120. :math:`\log_{30}8 = \log_{30}2^3 = 3\log_{30}2 = 3\log_{30}\frac{30}{15}`

     :math:`= 3\log_{30}30 - 3\log_{30}15 = 3 - 3(\log_{30}3 + \log_{30}5)`

     :math:`= 3(1 - a - b)`

121. Given, :math:`log_7 12 = a` and :math:`\log_{12} 24 = b`

     Multiplying :math:`ab = \log_724`

     Adding :math:`1` on both sides

     :math:`ab + 1 = \log_724 + \log_77 = \log_7168`

     Similarly, :math:`8a = \log_712^8` and :math:`5ab = \log_7168^5`

     :math:`\frac{ab + 1}{8a - 5ab} = \frac{\log_7168}{\log_712^8 - \log_7168^5}`

     Upong simplification we find that :math:`\log_{54}168 = \frac{ab + 1}{8a -
     5ab}`

122. **Case I:** When :math:`x > 1,` :math:`x > a^1 + 1.` Also, :math:`a^ + 1 <
     1 \therefore x > 1`

     **Case II:** When :math:`x < 1, x < a^2 + 1.` Also, :math:`a^2 > 0,
     \therefore x < 1`

     In both the cases :math:`x > 0`

123. Given :math:`\log_{12}18 = a` and :math:`\log_{24}54 = b`

     :math:`ab + 5(a - b) = \frac{\log 18}{\log 12}\frac{\log 54}{\log 24} +
     5\left(\frac{\log 18}{\log 12} - \frac{\log 54}{\log 24}\right)`

     :math:`=\frac{\log 18\log 54 + 5(\log 18\log 24 - \log 54\log 12)}{\log 12
     \log 24}`

     :math:`\log 18 = \log 2 + 2\log 3, \log 12 = 2\log 2 + \log 3, \\\log 24 =
     3\log 2 + \log 3, \log 54 = \log 2 + 3\log 3`

     Substituting and simplifying we obtain the desired result.

124. Since :math:`a, b, c` are in G.P.

     :math:`\Rightarrow b^2 = ac`

     Taking logarithm with base :math:`x,` we get

     :math:`2\log_x b = \log_x a + \log_x c`

     :math:`\frac{2}{\log_b x} = \frac{1}{\log_a x} + \frac{1}{\log_c x}`

     Thus, :math:`\log_a x, \log_b x, \log_c x` are in H.P.

125. Let :math:`r` be the common ratio of G.P. and :math:`d` be the common
     difference.

     :math:`\log a_n - b_n = \log a + n\log r - (b + nd) = \log a
     - b`

     :math:`n\log r - nd = 0`

     :math:`\log r = d`

     Thus, base :math:`b = r^\frac{1}{d}`

126. Given, :math:`\log_3 2, \log_3(2^x - 5)` and :math:`\log_3\left(2^x -
     \frac{7}{2}\right)` are in A.P.

     :math:`\therefore 2\log_3(2^x - 5) = \log_3\left(2^x -
     \frac{7}{2}\right) + \log_3 2`

     :math:`\Rightarrow (2^x - 5)^2 = 2\left(2^x - \frac{7}{2}\right)`

     Let :math:`z = 2^x,` then we have

     :math:`z^2 - 10z + 25 = 2z - 7`

     :math:`z^2 -12z + 32 = 0`

     :math:`z = \frac{12 \pm \sqrt{144 - 128}}{2} = 8, 4`

     :math:`\Rightarrow x = 2, 3`

     But if :math:`x = 2, 2^x - 5 < 0` so only acceptable value is :math:`x =
     3`

127. Let :math:`\log_2 7` is a rational number i.e. :math:`\log_2 7 =
     \frac{p}{q}` where :math:`p, q \in I`

     :math:`7 = 2^{\frac{p}{q}}\Rightarrow 7^q = 2^p`

     However, integral power of :math:`7` is odd but integral power of
     :math:`2` is even. Thus equality cannot hold and :math:`\log_2 7` cannot
     be rational i.e. it is irrational number.

128. Given, :math:`\log_{0.5}(x - 2) < \log_{0.25}(x - 2)`

     :math:`\Rightarrow (x - 2)^2 > (x - 2)`

     :math:`\Rightarrow (x - 2)(x - 3) > 0`

     Thus, :math:`x > 3` for logarithm function to be defined.
