Logarithm Solutions Part 2
**************************
51. Let :math:`x = 72^{15}~\therefore \log_{10}x = 15\log_{10}72`

    :math:`= 15\log_{10}(2^3*3^2) = 15[3\log_{10}2 + 2\log_{10}3]`

    :math:`= 15[3*0.301 + 2*0.477] = 15[0.903 + 0.954] = 15 * 1.857`

    :math:`= 27.855`

    So characteristic is :math:`27` the number of digits will be :math:`28`

52. Here we make use of the fact that number of integers with base :math:`b`
    and characteristics :math:`n` is :math:`b^{n + 1} - b^n.`

    Given :math:`b = 5, n = 2,` therefore number of integers is :math:`5^3 -
    5^2 = 100`

53. Let :math:`x = 3^{15}*2^{10}~\therefore \log_{10}x = 15\log_{10}3 +
    10\log_{10}2`

    :math:`= 15*0.477 + 10*0.301 = 7.155 + 3.01 = 10.165`

    Since characteritics is :math:`10` number of digits will be :math:`11`

54. Let :math:`x = 6^20~\therefore \log_{10}x = 20\log_{10}2*3`
    :math:`= 20[\log_{10}2 + \log_{10}3] = 20[0.301 + 0.477] = 20*0.778 = 15.56`

    Since characteristics is :math:`15` number of digits will be :math:`16`

55. Let :math:`x = 5^{25}~\therefore \log_{10}x = 25\log_{10}\frac{10}{2}`

    :math:`= 25[1 - \log_{10}2] = 25*0.699 = 17.475`

    Since characteristics is :math:`17` number of digits would be :math:`18`

56. :math:`\log_a [1 + \log_b \{1 + \log_c (1 + \log_p x)\}] = 0`

    :math:`1 + \log_b \{1 + \log_c (1 + \log_p x)\}] = 1`

    :math:`\log_b \{1 + \log_c (1 + \log_p x)\}] = 0`

    :math:`1 + \log_c (1 + \log_p x) = 1`

    :math:`\log_c (1 + \log_p x) = 0`

    :math:`1 + \log_p x = 1`

    :math:`\log_p x = 0`

    :math:`x = 1`

57. Given, :math:`\log_7\log_5(\sqrt{x + 5} + \sqrt{x}) = 0`

    :math:`\log_5(\sqrt{x + 5} + \sqrt{x}) = 1`

    :math:`\sqrt{x + 5} + \sqrt{x} = 5`

    :math:`\sqrt{x + 5} = 5 - \sqrt{x}`

    Squaring both sides, we get

    :math:`x + 5 = 25 + x -10\sqrt{x}`

    :math:`\sqrt{x} = 2~\Rightarrow x = 4`

58. :math:`\log_2 x + \log_4 (x + 2) = 2`

    :math:`\log_2 x + \log_{2^2} (x + 2) = 2`

    :math:`\log_2 x + \frac{1}{2}\log_2 (x + 2) = 2`

    :math:`2\log_2 x + \log_2 (x + 2) = 4`

    :math:`\log_2 x^2(x + 2) = 4`

    :math:`x^2(x + 2) = 16~\Rightarrow x = 2`

59. :math:`\log_(x + 2)x + \log_x (x + 2) = \frac{5}{2}`

    :math:`\frac{1}{\log_x(x + 2)} + \log_x(x + 1) = \frac{5}{2}`

    Let :math:`z = \log_x(x + 2)`

    :math:`\therefore \frac{1}{z} + z = \frac{5}{2}`

    :math:`2z^2 + 2 - 5z = 0\Rightarrow z = 2, \frac{1}{2}`

    :math:`\log_x(x + 2) = 2, \log_x(x + 2) = \frac{1}{2}`

    :math:`x + 2 = 2^x, x + 2 = \sqrt{x}`

    :math:`x = 2, x^2 - 3x + 4 = 0\Rightarrow x = \frac{3 \pm \sqrt{-7}}{2}`

    :math:`\therefore x = 2`

60. :math:`\frac{\log (x + 1)}{\log x} = 2`

    :math:`\log_x(x + 1) = 2`

    :math:`x + 1 = x^2 \Rightarrow x = \frac{1 \pm \sqrt{5}}{2}`

    :math:`\because x > 0, x = \frac{1 + \sqrt{5}}{2}`

61. :math:`2\log_x a + \log_{ax} a + 3\log_{a^2x} a = 0`

    :math:`\frac{2}{\log_a x} + \frac{1}{\log_a ax} + \frac{3}{\log_a a^2x} =
    0`

    :math:`\frac{2}{\log_a x} + \frac{1}{\log_a a + \log_a x} + \frac{3}{\log_a
    a^2 + \log_a x} = 0`

    :math:`\frac{2}{\log_a x} + \frac{1}{1 + \log_a x} + \frac{3}{2 + \log_a x}
    = 0`

    Let :math:`\log_a x = z,` so the above equation becomes

    :math:`\frac{2}{z} + \frac{1}{z + 1} + \frac{3}{z + 2} = 0`

    :math:`2(z + 1)(z + 2) + z(z + 2) + 3z(z + 1) = 0`

    :math:`2z^2 + 6z + 4 + z^2 + 2z + 3z^2 + 3z = 0`

    :math:`6z^2 + 11z + 4 = 0`

    :math:`z = \frac{-11 \pm \sqrt{121 - 4.6.4}}{12} = \frac{-11 \pm 5}{12} =
    \frac{-1}{2}, \frac{-4}{3}`

    :math:`\therefore x = a^{\frac{-1}{2}}, a^{\frac{-4}{3}}`

62. :math:`x + \log_{10}(1 + 2^x) = x\log_{10}5 + \log_{10}6`

    :math:`\log_{10}10^x + \log_{10}(1 + 2^x) = \log_{10}5^x + \log_{10}6`

    :math:`\log_{10}10^x(1 + 2^x) = \log_{10}5^x*6`

    :math:`10^x(1 + 2^x) = 5^x*6`

    :math:`2^x(1 + 2^x) = 2*3`

    :math:`2^x = 2, 1 + 2^x = 3~\Rightarrow x = 1`

63.  :math:`x^{\frac{3}{4}(\log_2 x)^2 + \log_2x - \frac{5}{4}} = \sqrt{2}`

     Taking :math:`\log_2` of both sides

     :math:`\left(\frac{3}{4}(\log_2 x)^2 + \log_2x - \frac{5}{4}\right)\log_2
     x = \frac{1}{2}\log_2 2`

     :math:`\left(\frac{3}{4}(\log_2 x)^2 + \log_2x - \frac{5}{4}\right)\log_2
     x = \frac{1}{2}`

     Let :math:`z = \log_2 x`

     :math:`\left(\frac{3}{4}z^2 + z - \frac{5}{4}\right)z = \frac{1}{2}`

     Solving this cubic equation will lead to :math:`x = 2, \frac{1}{4},
     \frac{1}{\sqrt[3]{2}}`

64. Given, :math:`(x^2 + 6)^{\log_3 x} = (5x)^{\log_3 x}`

    :math:`\log_3x` has a possible value of :math:`0` in that case :math:`x =
    1`

    If :math:`\log_3x \neq 0`

    :math:`x^2 + 6 = 5x~\Rightarrow x = 2, 3`

65. Given :math:`(3 + 2\sqrt{2})^{x^2 - 6x + 9} + (3 - 2\sqrt{2})^{x^2 - 6x +
    9} = 6`

    :math:`3 + 2\sqrt{2} = \frac{1}{3 - 2\sqrt{2}}`

    :math:`(3 + 2\sqrt{2})^{x^2 - 6x + 9} + (3 + 2\sqrt{2})^{-(x^2 - 6x +
    9)} = 6`

    Let :math:`z = (3 + 2\sqrt{2})^{x^2 - 6x + 9}`

    :math:`z + \frac{1}{z} = 6`

    :math:`z = \frac{6 \pm \sqrt{36 - 4}}{2} = \frac{3 \pm 2\sqrt{2}}{}`

    Thus, :math:`x^2 - 6x + 9 = \pm 1`

    Thus, :math:`x = 2, 4` because other roots are irrational.

66. Given :math:`\log_8\left(\frac{8}{x^2}\right) \div (\log_8 x)^2 = 3`

    :math:`\log_8 8 - \log_8 x^2 = 3 (\log_8 x)^2`

    :math:`1 - 2\log_8x = 3(\log_8 x)^2`

    Let :math:`z = \log_8 x`

    :math:`1 - 2z = 3z^2`

    :math:`z = -1, \frac{1}{3}`

    :math:`x = 2, \frac{1}{8}`

67. Given :math:`\sqrt{\log_2 (x)^4} + 4\log_4\sqrt{\frac{2}{x}} = 2`

    :math:`\sqrt{\log_2 (x)^4} + 2\log_2\sqrt{\frac{2}{x}} = 2`

    :math:`\sqrt{4\log_2 x} + \log_2 \frac{2}{x} = 2`

    :math:`\sqrt{4\log_2 x} + 1 - \log_2 x = 2`

    Now we can assume :math:`\log_2 x = z` and solve leading to :math:`x = 2`

68. Given, :math:`2\log_{10}x - \log_x0.01 = 5`

    :math:`2\log_{10}x - \log_x(10)^{-2} = 5`

    :math:`2\log_{10}x + 2\log_x{10} = 5`

    :math:`2\log_{10}x + \frac{2}{\log_{10}x} = 5`

    Let :math:`z = \log_{10}x`

    :math:`2z + \frac{2}{z} = 5`

    :math:`2z^2 - 5z + 2 = 0`

    :math:`z = 2, \frac{1}{2}`

    :math:`x = 100, \sqrt{10}`

69. Given :math:`\log_{\sin x}2\log_{\cos x}2 + \log_{\sin x} 2 + \log_{\cos
    x}2 = 0`

    :math:`\log_{\sin x}2(\log_{\cos x}2 + 1) + \log_{\cos x}2 = 0`

    Taking log of both sides with base :math:`e`:

    :math:`\frac{\ln 2}{\ln \sin x}\left(\frac {\ln 2}{ln \cos x}
    +1\right)+\frac {\ln 2}{ln \cos x}=0`

    :math:`\frac{1}{\ln \sin x}\left(\frac {\ln 2}{\ln \cos x} +1\right)+\frac
    {1}{\ln \cos x} = 0`

    :math:`\frac{1}{\ln \sin x}\left(\frac {\ln 2}{ln \cos x} +1\right)=-\frac
    {1}{\ln \cos x}`

    :math:`\frac{1}{ln \sin x}(ln 2 +ln \cos x)=-1`

    :math:`\ln(\sin 2x) = 1`

    :math:`x = 2k\pi + \frac{\pi}{4}, k\in I`

70. Given :math:`2^{x + 3} + 2^{x + 2} + 2^{x + 1} = 7^x + 7^{x - 1}`

    :math:`2^{x + 1}*7 = 7^{x - 1}* 8`

    :math:`(x + 1)\log 2 + \log 7 = (x - 1)\log 7 + 3\log 2`

    Solving this we get :math:`x = 2`

71. Given :math:`\log_{\sqrt{2}\sin x}(1 + \cos x) = 2`

    :math:`1 + \cos x = (\sqrt{2}\sin x)^2`

    :math:`1 + \cos x = 2\sin^2 x = 2 - 2\cos^2 x`

    :math:`2\cos^2 x + \cos x -1 = 0`

    :math:`\cos x = \frac{-1\pm \sqrt{1 + 8}}{4} = -1, \frac{1}{2}`

    :math:`x = 2n\pi, 2n\pi + \frac{\pi}{3},~n\in I`

    However, for logarithm to be defined :math:`\sin x > 0` therefore :math:`x
    = 2n\pi` is not an acceptable solution.

72. Given :math:`\log_{10}[198 + \sqrt{x^3 - x^2 - 12x + 36}] = 2`

    :math:`98 + \sqrt{x^3 - x^2 - 12x + 36} = 100`

    :math:`x^3 - x^2 - 12x + 32 = 0`

    Solving this we find one appropriate root which is :math:`x = -4`

73. Given :math:`2^x3^{2x} - 100 = 0`

    :math:`x\log_{10}2 + 2x\log_{10}3 = 2`

    Substituting valuues for :math:`\log_{10}2` and :math:`\log_{10}3,` we get

    :math:`0.30103x + 0.95424x = 2`

    :math:`x = 10593`

74. Give, :math:`\log_x 3\log_{\frac{x}{3}}3 + \log{\frac{x}{81}}3 = 0`

    :math:`\frac{1}{\log_3 x} + \frac{1}{\log_3\left(\frac{x}{3}\right)} +
    \frac{1}{\log_3}\left(\frac{x}{81}\right) = 0`

    :math:`\frac{1}{\log_3 x}.\frac{1}{\log_3 x - \log_3 3} + \frac{1}{\log_3 x
    - \log_3 81} = 0`

    Let :math:`z = \log_3 x`

    :math:`\frac{1}{z}.\frac{1}{z - 1} + \frac{1}{z - 4} = 0`

    :math:`z^2 - 4 = 0, z = \pm 2`

    :math:`x = 9, \frac{1}{9}`

75. Given, :math:`\log_{(2x + 3)}(6x^2 + 23x + 21) = 4 - \log_{(3x + 7)}(4x^2 +
    12x + 9)`

    :math:`\log_{(2x + 3)}(2x + 3)(3x + 7) = 4 - \log_{(3x + 7)}(2x + 3)^2`

    :math:`1 + \log_{(2x + 3)}(3x + 7) = 4 - 2\log_{(3x + 7)}(2x + 3)`

    Let :math:`z = \log_{(2x + 3)}(3x + 7)`

    :math:`1 + z = 4 - \frac{2}{z}`

    :math:`z = 1, 2~\Rightarrow x = -4, -2, \frac{-1}{4}`

    For logarithm to be defined :math:`2x + 3 > 0, 2x + 3 \neq 1`
    and :math:`3x + 7> 0, 3x + 7 \neq 1`

    Thus, :math:`x = -\frac{1}{4}` is the only valid solution.

76. Given :math:`\log_2(x^2 - 1) = \log_{\frac{1}{2}}(x - 1)`

    :math:`\log_2(x^2 - 1) = \log_{2^{-1}}(x - 1)`

    :math:`\log_2(x^2 - 1) = -\log_2(x - 1) = \log_2(x - 1)^{-1}`

    :math:`\log_2(x^2 - 1) = \log_2\frac{1}{x - 1}`

    :math:`x^2 - 1 = \frac{1}{x - 1}`

    :math:`x=0, x^2 - x - 1 = 0 \Rightarrow x= 0, \frac{1\pm \sqrt{5}}{2}`

    For logarithm to be defined :math:`x^2 - 1 > 0` and :math:`x - 1 > 0`

    Thus, :math:`x = \frac{1 + \sqrt{5}}{2}` is the only acceptable solution.

77. Given :math:`\log_5\left(5^{\frac{1}{x} + 125}\right) = \log_5 6 + 1 +
    \frac{1}{2x}`

    :math:`\log_5\left(5^{\frac{1}{x} + 125}\right) - \log_5 6 = 1 +
    \frac{1}{2x}`

    :math:`\log_5\left(\frac{5^{\frac{1}{x} + 125}}{6}\right) = 1 +
    \frac{1}{2x}`

    :math:`\frac{5^{\frac{1}{x} + 125}}{6} = 5^{1 + \frac{1}{2x}}`

    :math:`5^{\frac{1}{x}} + 125 = 20.5^{\frac{1}{2x}}`

    Let :math:`z = 5^{\frac{1}{x}}`

    :math:`z^2 - 30z + 125 = 0`

    :math:`z = 5, 25~\Rightarrow x = \frac{1}{2}, \frac{1}{4}`

78. For :math:`\log_{100}|x + y| = \frac{1}{2}`

    :math:`(x + y)^2 = 100`

    For and :math:`\log_{10} y - \log_{10}|x| = \log_{100} 4`

    :math:`\log_{10}\frac{y}{|x|} = \log_{10}2`

    :math:`y = 2|x|~\Rightarrow y^2 = 4x^2`

    Thus, we get :math:`5x^2 + 4x|x| = 100`

    When :math:`x > 0, x = \frac{10}{3}`

    When :math:`x < 0, x = -10`

    :math:`y = \frac{20}{3}, 20`

79. Given, :math:`2\log_2\log_2 x + \log_{\frac{1}{2}}\log_2(2\sqrt{2}x) = 1`

    :math:`\log_2(\log_2 x)^2 - \log_2\log_2(2\sqrt{2}x) = 1`

    :math:`\log_2 \left(\frac{(\log_2 x)^2}{\log_2 (2\sqrt{2}x)}\right) = 1`

    :math:`\frac{(\log_2 x)^2}{\log_2 (2\sqrt{2}x} = 2`

    :math:`(\log_ x)^2 = = \log_2(2\sqrt{2}x)`

    :math:`(\log_2 x)^2 - 3 - 2\log_2 x = 0`

    :math:`z^2 -2z - 3 = 0` where :math:`z = \log_2`

    :math:`z = -1, 3`

    :math:`\Rightarrow x = \frac{1}{2}, 8`

    For log to be defined :math:`x > 0` and :math:`2\sqrt{2}x > 0`

    :math:`\log_2 x > 0, \log_2 2\sqrt{2}x > 0`

    Thus, :math:`x = 8` is only acceptable solution.

80. Given :math:`\log_{\frac{3}{4}}\log_8(x^2 + 7) +
    \log_{\frac{1}{2}}\log_{\frac{1}{4}}(x^2 + 7)^{-1} = -2`

    :math:`\Rightarrow \log_{\frac{3}{4}}\log_{2^3}(x^2 + 7) +
    \log_{\frac{1}{2}}\log_{2^{-4}}(x^2 + 7)^{-1} = -2`

    :math:`\Rightarrow \log_{\frac{3}{4}}\left[\frac{1}{3}\log_2(x^2 +
    7)\right] + \log_{\frac{1}{2}}\left[\frac{1}{2}\log_2(x^2 + 7)\right] = -2`

    Let :math:`y = \log_2(x^2 + 7),` then we have

    :math:`\log_{\frac{3}{4}}\left(\frac{y}{3}\right) +
    \log_{\frac{1}{2}}\frac{1}{2} + \log_{\frac{1}{}}y = -2`

    :math:`\Rightarrow \log_{\frac{3}{4}}y - \log_{\frac{3}{4}}3 + 1+ 
    \log_{2^{-1}}y = -2`

    :math:`\Rightarrow \log_2y\left(\log_{\frac{3}{4}}2 - 1\right) = -3 +
    \log_{\frac{3}{4}} 3`

    Solving this we get :math:`\log_2 y = 2 \Rightarrow y = 4`

    :math:`x = \pm 3,` both of these values are valid for logarithm.

81. Given, :math:`\log_{10}x + \log_{10}x^{\frac{1}{2}} + \log_{10}x^{\frac{1}{4}}
    \ldots` to :math:`\infty = y`

    :math:`\log_{10}x\left[1 + \frac{1}{2} +
    \frac{1}{4}~\text{to}~\infty\right] = y`

    :math:`\log_{10}x \frac{1}{1 - \frac{1}{2}} = y \Rightarrow \log_{10}x =
    \frac{y}{2}`

    Also, given that

    :math:`\frac{1 + 3 + 5 + \ldots + (2y - 1)}{4 + 7 + 10 + \ldots + (3y + 1)}
    = \frac{20}{7\log_10 x}`

    :math:`\Rightarrow \frac{\frac{y}{2}[2 + (y - 1)2]}{\frac{y}{2}[8 + (y -
    1)3]} = \frac{20}{7\log_{10} x}`

    :math:`\frac{2y}{3y + 5} = \frac{20}{7\log_{10} x}`

    Thus, :math:`\frac{2y}{3y + 5} = \frac{20\times 2}{7y}`

    :math:`\Rightarrow 7y^2 - 60y -100 = 0`

    :math:`y = 10, \frac{-10}{7}`

    Since number of terms cannot be a fraction, therefore :math:`y = 10` is the
    answer. Hence, :math:`x = 10^5`

82. Given, :math:`18^{4x - 3} = (54\sqrt{2})^{3x - 4}`

    Taking log on both sides,

    :math:`(4x - 3)\log 18 = (3x - 4)log(18.3\sqrt{2})`

    :math:`\Rightarrow (4x - 3)\log 18 = (3x - 4)\log 18^{\frac{3}{2}}`

    :math:`\Rightarrow 4x - 3 = (3x - 4)\frac{3}{2}`

    :math:`\Rightarrow x = 6`

83. Given, :math:`4^{\log_9 3} + 9^{\log_2 4} = 10^{\log_x 83}`

    :math:`\Rightarrow 4^{\log_{3^2} 3 + 9^{\log_2 2^2}} = 10^{\log_x 83}`

    :math:`\Rightarrow 4^{\frac{1}{2}\log_3 3} + 9^{2\log_2 2} = 10^{\log_x
    83}`

    :math:`\Rightarrow 4^\frac{1}{2} + 9^2 = 10^{\log_x 83}`

    :math:`\Rightarrow 83 = 10^{\log_x 83}`

    :math:`x = 10`

84. Given, :math:`3^{4\log_9 (x + 1)} = 2^{2\log_2 (x + 3)}`

    :math:`\Rightarrow 3^{2\log_3 (x + 1)} = x^2 + 3 [\because a^{\log_a N} =
    N]`      

    :math:`\Rightarrow 3^{\log_3 (x + 1)^2} = x^2 + 3`

    :math:`\Rightarrow x^2 + 2x + 1 = x^2 + 3`

    :math:`\Rightarrow x = 1`

85. Given, :math:`\frac{6}{5}a^{\log_a x\log_{10} a \log_a 5} -
    3^{\log_{10}\left(\frac{x}{10}\right)} = 9^{\log_{100}x + \log_4 2}`

    :math:`\Rightarrow \frac{6}{5}a^{\log_{10}x\log_a 5}- 3^{\log_{10}{x - 1}}
    = 9^{\frac{1}{2}\log_{10} x + \frac{1}{2}\log_2 2}`

    :math:`\Rightarrow \frac{6}{5}\left(a^{\log_a 5}\right)^{\log_{10} x} -
    3^{\log_{10}{x - 1}} = 3\log_{10}^{x + 1}`

    :math:`\Rightarrow \frac{6}{5}5^{\log_{10}x} = 3^{\log_{10}{x + 1}} +
    3^{\log_{10}{x + 1}}`

    :math:`\Rightarrow 6.5^{\log_{10}{x - 1}} = 3^{\log_{10}{x - 1}}.(1 + 3^2)`

    :math:`\Rightarrow \left(\frac{5}{3}\right)^{\log_{10}{x - 1}} =
    \frac{10}{6}`

    :math:`\Rightarrow \log_{10} x - 1 = 1\Rightarrow x = 100`

86. Given, :math:`2^{3x + \frac{1}{2}} + 2^{x + \frac{1}{2}} = 2^{\log_2 6}`

    :math:`2^{3x}\sqrt{2} + 2^x\sqrt{2} = 6`

    :math:`(2^x)^3 + 2^x = 3\sqrt{2}`

    Let :math:`z = 2^x,` then we can rewrite above as

    :math:`z^3 + z = 3\sqrt{2}`

    :math:`z = \sqrt{2}, \frac{-\sqrt{2}\pm \sqrt{2 - 12}}{2}`

    Ignoring complex roots we have :math:`z = \sqrt{2}`

    :math:`\therefore 2^x = \sqrt{2}`

    :math:`x = \frac{1}{2}`

87. Given, :math:`(5 + 2\sqrt{6})^{x^2 - 3} + (5 - 2\sqrt{6})^{x^2 - 3} = 10`

    :math:`\Rightarrow (5 + 2\sqrt{6})^{x^2 - 3} + (5 + 2\sqrt{6})^{-(x^2 - 3)}
    = 10`

    Let :math:`z = (5 + 2\sqrt{6})^{x^2 - 3},` then we can rewrite above as

    :math:`z + \frac{1}{z} = 10`

    :math:`z = 5\pm 2\sqrt{6}`

    :math:`\therefore x = \pm 2, \pm\sqrt{2}`

88. :math:`2\log_{10}x - \log_x .01 = 2\log_{10}x - \log_x 10^{-2}`

    :math:`= 2\log_{10}x + 2\log_x 10 = 2\log_{10}x + 2\frac{1}{\log_{10}x}`

    :math:`= 2\left(\log_{10}x + \frac{1}{\log_{10}x}\right)`

    Let :math:`z = \log_{10}x,` then above can be rewritten as

    :math:`= 2\left(z + \frac{1}{z}\right)`

    :math:`= 2\left[\left(\sqrt{z} - \frac{1}{\sqrt{z}}\right)^2 + 2\right]
    \geq 4`

    Thus, given condition is proved.

89. Let :math:`E = \log_b a + \log_a b = \log_b a + \log_a b`

    Also, let :math:`z = \log_b a,` then we can rewrite above as

    :math:`E = z + \frac{1}{z}`

    Clearly, :math:`z \neq 0,` or the problem will be undefined.

    When :math:`z > 0, E = z + \frac{1}{z} = \left(\sqrt{z} -
    \frac{1}{\sqrt{z}}\right)^2 + 2 > 2`

    When :math:`z < 0,` let :math:`z = -y,` then we have

    :math:`E = \left|z + \frac{1}{z}\right| = \left|-y - \frac{1}{y}\right|`

    :math:`= y + \frac{1}{y} > 2`

90. Given, :math:`\log_{0.3}(x ^2 + 8) > \log_{0.3}9x`

    :math:`x^2 + 8 < 9x`

    :math:`\Rightarrow 1 < x < 8`

91. Given, :math:`\log_{x - 2}(2x - 3) > \log(x - 2)(24 - 6x)`

    **Case I:** When :math:`0 < x - 2 < 1, \Rightarrow 2 < x < 3`

    Given inequality becomes :math:`2x - 3 < 24 - 6x\Rightarrow x < \frac{27}{8}`

    But :math:`x < 3` so :math:`3` is still limiting value of :math:`x`

    **Case II:** When :math:`x - 2 > 1, \Rightarrow x > 3`

    Given inequality becomes :math:`2x - 3 > 24 - 6x\Rightarrow x > \frac{27}{8}`

    However, for logarithm function to be defined :math:`2x - 3 > 0` and
    :math:`24 - 6x > 0` and also :math:`x - 2 > 0`

    Combining all these we get :math:`2 < x < 3`

92. Given :math:`\log_{0.3}(x - 1) < \log_{0.09}(x - 1)`

    :math:`\Rightarrow (x - 1)^2 > (x - 1)`

    :math:`\Rightarrow x^2 - 3x + 2 > 0`

    :math:`\Rightarrow x < 1, x> 2`

    For logarithm functiton to be defined :math:`x > 1,` thus the interval for
    :math:`x` would be :math:`(2, \infty]`

93. Given, :math:`\log_{\frac{1}{2}}x \geq \log_{\frac{1}{3}}x`

    :math:`\Rightarrow \log_{\frac{1}{2}}x \geq \log_{\frac{1}{2}}x
    \log_{\frac{1}{3}} \frac{1}{2}`

    :math:`\Rightarrow \log_{\frac{1}{2}}x\left[1 -
    \log_{\frac{1}{3}}\frac{1}{2}\right] \geq 0`

    :math:`\Rightarrow \log_{\frac{1}{2}}x\left[1 - \log_{3^{-1}}(2^{-1})\right] \geq
    0`

    :math:`\Rightarrow \log_{\frac{1}{2}}x[1 - \log_3 2] \geq 0`

    :math:`\Rightarrow \log_{\frac{1}{2}}x \geq 0`

    :math:`\Rightarrow x \leq 1`

    For logarithm function to be defined :math:`x > 0,` thus range of :math:`x`
    would be :math:`(0, 1]`

94. Given, :math:`\log_{\frac{1}{3}}\log_4(x^2 - 5) > 0`

    :math:`\log_4(x^2 - 5) < 1`

    For logarithm ot be defined :math:`x^2 - 5 > 0` and :math:`\log_4 (x^2 - 5)
    > 0`

    Combining all these conditions we get two ranges for :math:`x, (-3,
    -\sqrt{6})` and :math:`(\sqrt{6}, 3)`

95. Given, :math:`\log (x^2 - 2x - 2)\leq 0`

    :math:`\Rightarrow x^2 -2x -2 \leq 1`

    :math:`\Rightarrow -1 \leq x \leq 3`

    For logarithm function to be defined :math:`x^2 - 2x - 2 > 0`

    :math:`x < 1 - \sqrt{3}, x > 1 + \sqrt{3}`

    Combining these ranges gives us the interval of values in which :math:`x`
    can lie.

96. Given, :math:`\log_2^2(x - 1)^2 - \log_{0.5}(x - 1) > 5`

    :math:`\Rightarrow (2\log_2|x - 1|)^2 - \log_{\frac{1}{2}}(x - 1) > 5`

    :math:`\Rightarrow 4[\log_2 (x - 1)]^2 + \log_2(x - 1) > 5`

    Let :math:`z = \log_2 (x - 1)`

    :math:`\Rightarrow 4z^2 + z - 5 > 0`

    :math:`\Rightarrow z < \frac{-5}{4}, x > 1`

    When :math:`z < \frac{-5}{4}, x - 1 < 2^{\frac{-5}{4}}\Rightarrow x < 1 +
    \frac{1}{2\sqrt[4]{2}}`

    For log to be defined :math:`x - 1 > 0, x > 1`

    When :math:`z > 1, x  > 3`

    Thus range of :math:`x` is :math:`\left(1, 1 +
    \frac{1}{2\sqrt[4]{2}}\right)\cup (3, \infty)`

97. Let :math:`E = \log_2 17\log{\frac{1}{5}} 2\log_3\frac{1}{5} > 2`

    :math:`L.H.S. = \log_2 17\log_3 2 = \log_3 17`

    :math:`\because 17 > 3^2`

    :math:`\therefore \log_3 17 > 2`

98. We have to prove that :math:`\frac{1}{3} < \log_{20} 3 < \frac{1}{2}`

    :math:`\frac{1}{3} < \log_{20} 3\Rightarrow 1< 3\log_{20}3`

    :math:`\Rightarrow 1 < \log_{20} 3^3\Rightarrow 1 < \log_{20} 27`

    which is true as base is greater than :math:`1` and number is greater than
    base.

    :math:`\log_{20} 3 < \frac{1}{2}\Rightarrow 2\log_{20} 3 < 1`

    :math:`\Rightarrow \log_{20} 3^2 < 1\Rightarrow \log_{20} 9 < 1`

    which is true because number is less than base.

99. We have to prove that :math:`\frac{1}{4} < \log_{10} 2 < \frac{1}{2}`

    Taking first two parts, :math:`\frac{1}{4} < \log_{10}2`

    :math:`\Rightarrow 1 < 4\log_{10} 2 = \log_{10} 2^4 = \log_{10}16`

    which is true because :math:`10 > 1` and number is greater than base.

    Taking last two parts, :math:`\log_{10} 2 < \frac{1}{2}`

    :math:`\Rightarrow 2\log_{10} 2 < 1\Rightarrow \log_{10}2^2 < 1`

    :math:`\Rightarrow \log_{10} 4 < 1`

    which is true because :math:`10 > 1` and number is samllers than base.

100. Given, :math:`\log_{0.1}(4x^2 - 1) > \log_{0.1}3x`

     :math:`4x^2 - 3x - 1 < 0`

     :math:`(4x + 1)(x - 1) < 0`

     Thus, :math:`[-\infty, -\frac{1}{4})\cup(1, \infty]` is initial solution.

     Now, :math:`x > 0` is another restriction from R.H.S.

     From L.H.S. :math:`4x^2 - 1 > 0`

     :math:`\Rightarrow x < -\frac{1}{2}, x > \frac{1}{2}`

     Combining all these we get, :math:`\frac{1}{2} < x < 1`
