.. meta::
   :author: Shiv Shankar Dayal
   :title: Quadratic Equations Solutions Part 6
   :description: Quadratic Equations Solutions Part 6
   :keywords: quadratic equations, algebra

Quadratic Equations Solutions Part 6
************************************
251. :math:`D = c^2(3a^2 + b^2)^2 + 4abc^2(6a^2 + ab - 2b^2)`

     :math:`= c^2(9a^4 + b^4 + 6a^2b^2 + 4a^3b + 4a^2b^2 - 8ab^3)`

     :math:`= c^2(3a^2 - b^2 + 4ab)^2`

     which is a perfect square and hence roots are rational.
252. :math:`\sqrt{\frac{m}{n}} + \sqrt{\frac{n}{m}} + \frac{b}{\sqrt{ac}} = 0`

     :math:`L. H. S. = \sqrt{\frac{\alpha}{\beta}} + \sqrt{\frac{\beta}{\alpha}} + \frac{b}{\sqrt{ac}}`

     :math:`= \frac{\alpha + \beta}{\sqrt{\alpha\beta}} + \frac{b}{\sqrt{ac}}`

     :math:`= \frac{-\frac{b}{a}}{\sqrt{\frac{c}{a}}} + \frac{b}{\sqrt{ac}} = 0`
253. Let :math:`\alpha` be the root, then the second root would be :math:`\alpha^3`.

     Product of roots :math:`= \alpha^4 = a \Rightarrow \alpha = a^{\frac{1}{4}}`

     Sum of roots :math:`= \alpha + \alpha^3 = -f(a)`

     :math:`\Rightarrow f(a) = -a^{\frac{1}{4}} - a^{\frac{3}{4}}`

     Therefore, the general equation in :math:`x` would be

     :math:`f(x) = -x^{\frac{1}{4}} - x^{\frac{3}{4}}`
254. Since :math:`\alpha, \beta` are roots of the equation :math:`x^2 - px + q = 0` therefore

     :math:`\alpha + \beta = p` and :math:`\alpha\beta = q`

     :math:`(\alpha^2 - \beta^2)(\alpha^3 - \beta^3) = (\alpha - \beta)^2(\alpha + \beta)[(\alpha + \beta^2) - \alpha\beta]`

     :math:`=(p^2 - 4q)p(p^2 - q)`

     :math:`\alpha^3\beta^2 + \alpha^2\beta^3 = \alpha^2\beta^2(\alpha + \beta) = pq^2`

     Therefore, the equation would be

     :math:`x^2 - p[(p^2 - 4q)(p^2 - q) + q^2]x + p^2q^2(p^2 - 4q)(p^2 - q) = 0`
255. This problem has been left as an exercise.
256. Let :math:`\alpha, \beta` be the roots then :math:`\alpha + \beta = -\frac{b}{a}` and :math:`\alpha\beta = \frac{c}{a}`

     According to the question :math:`\alpha + \beta = \frac{1}{\alpha^2} + \frac{1}{\beta^2}`

     :math:`-\frac{b}{a} = \frac{(\alpha + \beta)^2 - 2\alpha\beta}{\alpha^2\beta^2}`

     :math:`-\frac{b}{a} = \frac{\frac{b^2}{a^2}}{\frac{c^2}{a^2}} - 2\frac{1}{\frac{c}{a}}`

     :math:`-\frac{b}{a} = \frac{b^2}{c^2} - 2\frac{a}{c}`

     :math:`\Rightarrow \frac{b^2}{ac} + \frac{bc}{a^2} = 2`
257. Given, :math:`T = 2\pi \sqrt{\frac{h^2 + k^2}{gh}}`

     Squaring, :math:`h^2 + k^2 = \frac{T^2gh}{4\pi^2}`

     :math:`h^2 - \frac{T^2gh}{4\pi^2} + k^2 = 0`

     Clearly, :math:`h_1` and :math:`h_2` are two possible roots of above equation where

     :math:`h_1 + h_2 = \frac{T^2g}{4\pi^2}` and :math:`h_1h_2 = k^2`
258. Clearly, :math:`\alpha_1 + \alpha_2 = -p` and :math:`\alpha_1\alpha_2 = q`

     :math:`\beta_1 + \beta2 = -r` and :math:`\beta_1\beta_2 = s`

     Solving the two equations in :math:`y` and :math:`z` by elimination we have

     :math:`\frac{\alpha_1}{\alpha_2} = \frac{\beta_1}{\beta_2} = k`

     :math:`\frac{p^2}{r^2} = \frac{(\alpha_1 + \alpha_2)^2}{(\beta_1 + \beta_2)^2}`

     :math:`= \frac{\alpha_1^2(1 + k^2)}{\beta_1(1 + k^2)} = \frac{\frac{\alpha_1\alpha_2}{k}}{\frac{\beta_1\beta_2}{k}} = \frac{q}{s}`
259. :math:`-(1 + \alpha\beta) = -(\frac{a + c}{a})`

     H. M. of :math:`\alpha` and :math:`\beta = \frac{2\alpha\beta}{\alpha + \beta} = -\frac{2c}{b}`

     but since :math:`a, b, c` are in H. P. it becomes

     :math:`= -\frac{2c}{\frac{2ac}{a + c}} = -(\frac{a + c}{a}) = -(1 + \alpha\beta)`
260. Given equation is :math:`x + 1 = \lambda x - \lambda^2x^2`

     :math:`\lambda^2x^2 + (1 - \lambda)x + 1 = 0`

     :math:`\Rightarrow \alpha + \beta = \frac{\lambda - 1}{\lambda^2}` and :math:`\alpha\beta = \frac{1}{\lambda^2}`

     Also given that, :math:`\frac{\alpha}{\beta} + \frac{\beta}{\alpha} = r - 2`

     :math:`\Rightarrow \alpha^2 + \beta^2 = (r - 2)\alpha\beta`

     :math:`(\alpha + \beta)^2 = r\alpha\beta`

     :math:`\frac{(\lambda - 1)^2}{\lambda^4} = \frac{r}{\lambda^2}`

     :math:`\Rightarrow \lambda_1 + \lambda_2 = \frac{2}{1 - r}` and :math:`\lambda_1\lambda_2 = \frac{1}{1 - r}`

     Now substituting and solving we get the desired result.
261. Let :math:`\alpha, \beta` be roots of :math:`ax^2 + bx + c = 0` then

     :math:`\alpha + \beta = -\frac{b}{a}` and :math:`\alpha\beta = \frac{c}{a}`

     According to question, :math:`\frac{1}{\alpha} + \frac{1}{\beta} = -\frac{m}{l}` and :math:`\frac{1}{\alpha\beta} = \frac{n}{l}`

     From product of roots, :math:`\frac{c}{a} = \frac{l}{n}` and from sum of roots :math:`\frac{b}{c} = \frac{m}{l}`

     Hence the relation is established.
262. Let the roots are :math:`l, lm, lm^2, lm^3` which is an increasing G. P.

     Sum of roots for first equation :math:`= l(1 + m) = 3`

     Sum of roots for second equation :math:`= lm^2(1 + m) = 12 \Rightarrow m^2 = 4 \Rightarrow m = 2` because G. P. is
     increasing.

     :math:`\Rightarrow l = 1`

     :math:`A = l^2m = 2` and :math:`B = l^2m^5 = 32`
263. For first equation, :math:`p + q = 2` and :math:`pq = A.` For second equation, :math:`r + s = 18` and :math:`rs =
     B`

     Let :math:`a` be the first term and :math:`d` be the common difference, then

     :math:`p = a - 3d, q = a - d, r = a + d, s = a + 3d`

     Substituting in sums we have :math:`2a - 4d = 2` and :math:`2a + 4d = 18`

     :math:`\therefore a = 5` and :math:`d = 2`

     :math:`\therefore p = -1, q = 3, r = 7, s = 11`

     :math:`\therefore A = -3` and :math:`B = 77`
264. :math:`\alpha + \beta = -a` and :math:`\alpha\beta = -\frac{1}{2a^2}`

     :math:`\alpha^4 + \beta^4 = ((\alpha + \beta)^2 - 2\alpha\beta)^2 - 2\alpha^2\beta^2`

     :math:`= 2 + a^4 + \frac{1}{2a^4}`

     Let :math:`a^4 + \frac{1}{2a^4} = y`

     :math:`\Rightarrow 2a^8 - 2a^4y - 1 = 0`

     Since :math:`a` is real. :math:`\therefore y^2 - 2 \ge 0 \Rightarrow y \ge \sqrt{2} [\because a^4 \ge 0]`

     :math:`\alpha^4 + \beta^4 \ge 2 + \sqrt{2}`
265. :math:`\alpha + \beta = p` and :math:`\alpha\beta = q`

     :math:`\alpha^{\frac{1}{4}} + \beta^{\frac{1}{4}} = \sqrt[4]{\left(\alpha^{\frac{1}{4}} +
     \beta^{\frac{1}{4}}\right)^4}`

     :math:`= \sqrt[4]{\alpha + \beta + 6\sqrt{\alpha\beta} + 4\sqrt[4]{\alpha\beta(\alpha^2 + \beta^2)}}`

     :math:`= \sqrt[4]{p + 6\sqrt{q} + 4\sqrt[4]{q(p^2 - 2q)}}`
266. Let :math:`\alpha, beta` be roots of first equation and :math:`\gamma, \delta` be that of second equation.

     :math:`\alpha + \beta = \frac{b}{a}, \alpha\beta = \frac{c}{a}` and :math:`\gamma + \delta = \frac{c}{b},
     \gamma\delta = \frac{a}{b}`

     According to question, :math:`\alpha - \beta = \gamma - \delta`

     :math:`(\alpha + \beta)^2 - 4\alpha\beta = (\gamma + \delta)^2 - 4\gamma\delta`

     :math:`\frac{b^2}{a^2} - \frac{4c}{a} = \frac{c^2}{b^2} - \frac{4a}{b}`

     :math:`\Rightarrow b^4 - a^2c^2 = 4ab(bc - a^2)`
267. A cubic equation whose roots are :math:`\alpha, \beta, \gamma` is given by :math:`f(x) = (x - \alpha)(x -
     \beta)(x - \gamma)`

     :math:`\therefore f'(x) = (x - \alpha)(x - \beta) + (x - \beta)(x - \gamma) + (x - \alpha)(x - \gamma)`

     Now it is trivial to prove that a sign change occurs for the given limits for :math:`f'(x)` and thus a root lies in
     these limits.
268. Since :math:`\alpha, \beta, \gamma, \delta` are in A. P. let :math:`\alpha = l - 3m, \beta = l - m, \gamma = l + m,
     \delta = l + 3m` where :math:`l` is the first term and :math:`m` is the common difference of A. P.

     :math:`\alpha + \beta = -\frac{b}{a}, \alpha\beta = \frac{c}{a}` and :math:`\gamma + \delta = -\frac{q}{p},
     \gamma\delta = \frac{r}{p}`

     :math:`\frac{D_1}{D_2} = \frac{b^2 - 4ac}{q^2 - 4pr} = \frac{\frac{b^2}{a^2} - \frac{4c}{a}}{\frac{a^2}{p^2} -
     \frac{4r}{p}}\frac{a^2}{p^2}`

     :math:`= \frac{(\alpha - \beta)^2}{(\gamma - \delta)^2}\frac{a^2}{p^2} = \frac{4d^2}{4d^2}\frac{a^2}{p^2}`
269. This is similar to 268 and has been left as an exercise.
270. This is a very easy problem and has been left as an exercise.
271. :math:`\alpha + \beta = -\frac{b}{a}, \alpha\beta = \frac{c}{a}` and :math:`\alpha^4 + \beta^4 = -\frac{m}{l},
     \alpha^4\beta^4 = \frac{n}{l}`

     Discriminant of given quadratic equation, :math:`D = 16a^2c^2l^2 - 4a2^l(2c^2l + a^2m)`

     :math:`= 8a^2c^2l^2 - 4a^4lm`

     :math:`= 4a^4l^2\left(2\frac{c^2}{a^2} - \frac{m}{l}\right)`

     :math:`= 4a^4l^2(2\alpha^2\beta^2 + \alpha^4 + \beta^4) = 2a^4l^2(\alpha^2 + \beta^2)^2`

     Therefore, roots of the given equation can be computed which are found to be :math:`(\alpha + \beta)^2, -(\alpha +
     \beta)^2` which are equal and opposite in sign.
272. :math:`\alpha + \beta = -\frac{b}{a}, \alpha\beta = \frac{c}{a}` and :math:`\gamma + \delta = -\frac{m}{l},
     \gamma\delta = \frac{n}{l}`

     Equation whose roots are :math:`\alpha\gamma + \beta\delta` and :math:`\alpha\delta + \beta\gamma` is

     :math:`x^2 - (\alpha\gamma + \beta\delta + \alpha\delta + \beta\gamma)x + (\alpha\gamma +
     \beta\delta)(\alpha\delta + \beta\gamma) = 0`

     :math:`x^ - (\alpha + \beta)(\gamma + \delta)x + ((\alpha^2 + \beta^2)\gamma\delta + (\gamma^2 +
     \delta^2)\alpha\beta) = 0`

     :math:`a^2l^2x^2 - ablmx + (b^2 - 2ac)ln + (m^2 - 2ln)ac = 0`
273. :math:`p` and :math:`q` are roots of the equation :math:`3x^2 - 5x - 2 = 0`

     :math:`\Rightarrow p + q = \frac{5}{3}` and :math:`pq = -\frac{2}{3}`

     Equation whose roots are :math:`3p - 2q` and :math:`3q - 2p` is

     :math:`x^2 - (p + q)x - 6p^2 - 6q^2 + 13pq = 0`

     :math:`3x^2 - 5x - 100 = 0`
274. Since :math:`p` and :math:`q` are roots of the equation :math:`x^2 + bx + c = 0` therefore :math:`p + q = -b` and
     :math:`pq = c`

     Equation whose roots are :math:`b` and :math:`c` is

     :math:`x^2 - (b + c)x + bc = 0`

     :math:`x^2 +(p + q - pq)x - pq(p + q) = 0`
275. Sum of roots :math:`= 2\alpha = -p` and product of roots :math:`= \alpha^2 - \beta = q \Rightarrow \beta =
     \frac{p^2 - 4q}{4}`

     Equation whose roots are :math:`\frac{1}{\alpha}\pm \frac{1}{\sqrt{\beta}}` is

     :math:`x^2 - \frac{2}{\alpha}x + \frac{1}{\alpha^2} - \frac{1}{\beta} = 0`

     :math:`x^2 + \frac{2}{p}x + \frac{1}{p^2} - \frac{4}{p^2 - 4q} = 0`

     :math:`(p^2 - 4q)(p^2x^2 + 4px) = 16q`
276. Proceeding like previous problem the equation can be found as :math:`qx^2 - p(p^2 - q)(p^2 - 4q)x - p^2q^2(p^2 -
     4q) = 0`

Rest of the problems have been left as exercises.
