.. meta::
   :author: Shiv Shankar Dayal
   :title: Quadratic Equations Solutions Part 7
   :description: Quadratic Equations Solutions Part 7
   :keywords: quadratic equations, algebra

Quadratic Equations Solutions Part 7
************************************
301. :math:`f(11) = 1331 - 1210 - 121 - 100 < 0`

     :math:`f(12) = 1728 - 1440 - 132 - 100 > 0`

     :math:`f'(x) = 3x^2 - 20x - 11`

     Clearly, :math:`f'(x) > 0~\forall~x > 12`

     Therefore, :math:`f(x)` will have its greatest root between :math:`11` and :math:`12`. Hence, integral
     part of greatest root is :math:`11`.
302. :math:`f(0) = a_n` and :math:`f(1) = a_0 + a_1 + ... + a_n` which are both odd numbers.

     :math:`f(2k)=a_n+2(a_{n - 1}k)+2(2a_{n - 2}k^2)+\ldots +2(2^{n-1}k^na_n)` is odd for all :math:`k` and

     :math:`f(2k+1)=\sum_{k=1}^na_k\sum_{i=1}^k{k\choose i}(2k)^i`

     Since all the inner summands are even except when :math:`i = 0` we see that

     :math:`f(2k+1)=2N+\sum_{k=1}^na_k`

     which is even plus add i.e. odd for all values of :math:`k`.

     Thus, for no integer the function is zero hence the function has no integral roots.
303. Let :math:`g(x) = e^xf(x)` then :math:`g"(x) = e^x[f(x) + 2f'(x) + f"(x)]`

     Therefore, roots of :math:`g"(x) = 0` will be same as :math:`f(x) + 2f'(x) + f"(x) = 0` as :math:`e^x \ne 0`

     But since :math:`e^x \ne 0, g(x)` will have same roots as :math:`f(x).`

     Since :math:`f(x) = 0` has three roots :math:`\alpha < \beta < \gamma,` therefore equation :math:`g(x) = 0` will have same
     roots and :math:`g'(x) = 0` will have a root between :math:`\alpha` and :math:`\beta` and other roots between :math:`\beta`
     and :math:`\gamma` and hence :math:`g"(x)` will have a root between :math:`\alpha` and :math:`\gamma.`
304. If this degree four polynomial has four real roots, then there is a local minimum between the first two and between
     the last two roots, and a local maximum between the second and hird root. The location of the extrema does not
     change with :math:`a`, only their :math:`y` values. Thus we are looking for :math:`a` such that the two local
     minima have negative :math:`y` values and the local maximum has positive :math:`y` value.

     Locate the local extrema as roots of the derivative :math:`4x^3 - 12x^2 - 16x` which has roots as :math:`-1, 0, 4`

     :math:`\Rightarrow a = 0, a = 3, a = 128`

     :math:`\therefore 0\le a \le 3`
305. This problem is similar to 226 and can be solved similarly.
306. :math:`f'(x) = 5(x - 1)^4 + 7(x + 2)^6 + 9(7x - 5)^8` can never be zero for any real value of :math:`x` therefore
     the given equation can have only one real real root at maximum.
307. Let :math:`x + 2 = t^2` then :math:`\sqrt{2(t^2 + 1)} - t = 3 \Rightarrow 2t^2 + 2 = 9 + 6t + t^2`

     :math:`\Rightarrow t = 7, -1`

     Now it is trivial to calculate the values. 308 through 317 have been left as exercises.

318. :math:`\sum_{i = 1}^n(x - a_i)^2 = nx^2 - 2(a_1 + a_2 + ... + a_n)x + (a_1^2 + a_2^2 + ... + a_n^2)`

     This is a quadratic equation in :math:`x` and coefficient of :math:`x^2` is :math:`n > 0,` therefore this quadratic
     equation will have least value at :math:`x = \frac{a_1 + a_2 + ... + a_n}{n}`
319. Let the quotient be :math:`\frac{n}{n^2 - 1},` where :math:`n` is a natural number.

     According to question,

     :math:`\frac{n + 2}{n^2 - 1 + 2} > \frac{1}{3 \Rightarrow n^2 - 3n - 5 < 0}`

     :math:`\Rightarrow \frac{3}{2} - \frac{\sqrt{29}}{2} < n < \frac{3}{2} + \frac{\sqrt{29}}{2}`

     Also, :math:`0 < \frac{n - 3}{n^2 - 1 - 3} < \frac{1}{10}`

     :math:`\Rightarrow -2 < n < 2` or :math:`3 < n < \infty` or :math:`n > 2`

     :math:`n = 4` is the only natural number satisfying all the conditions. Therefore, quotient is
     :math:`\frac{4}{15}.`
320. Let :math:`f(x) = ax^2 + bx + c` then :math:`g(x) = ax^2 + (2a + b)x + c + b + 2a`

     Given, :math:`ax^2 + bx + c > 0` for all :math:`x` :math:`\therefore b^2 - 4ac < 0` and :math:`a > 0`

     Discriminant of :math:`g(x) = 0`

     :math:`D = (b + 2a)^2 - 4a(c + b + 2a) = b^2 - 4ac - 4a^2 < 0` and :math:`a > 0`

     Hence, :math:`g(x) > 0` for all :math:`x.`
321. Clearly, :math:`f(x) \ge 0` for all :math:`x` then :math:`D \le 0` because coefficient of :math:`x^2` is positive.

     :math:`4(a_1b_1 + a_2b_2 + ... + a_nb_n)^2 \le 4(a_1^2 + a_2^2 + ... + a_n^2)(b_1^2 + b_2^2 + ... + b_n^2)`

     Hence, proven.
322. Given equation is :math:`[(x+1)(x+m)][x(x+m+1)] = m^2`

     :math:`(x^2 + (m + 1)x + m)(x^2 + (m + 1)x) = m^2`

     :math:`(y + m)y = m^2` where :math:`y = x^2 + (m + 1)x`

     :math:`y^2 + my - m^2 = 0 \therefore y = \frac{-m \pm \sqrt{5}m}{2}`

     :math:`\Rightarrow x^2 + (m + 1)x = \frac{-m \pm \sqrt{5}m}{2}`

     These two equations must have real roots only then original will have four.
     Now it is trivially obtained that

     :math:`-\infty<m<-2-\sqrt{5}` or :math:`2 + \sqrt{5}<m<\infty` or :math:`2 - \sqrt{5}<m<-2+\sqrt{5}`
323. Given equation is :math:`x^4 + (a - 1)x^3 + x^2 + (a - 1)x + 1 = 0`

     Dividing both sides from :math:`x^2` we have

     :math:`x^2 + (a - 1)x + 1 + (a - 1)\frac{1}{x} + \frac{1}{x^2} = 0`

     :math:`\Rightarrow \left(x+\frac{1}{x}\right)^2 - 2x\frac{1}{x} + (a - 1)\left(x + \frac{1}{x}\right) + 1 = 0`

     :math:`\Rightarrow y^2 + (a - 1)y - 1 = 0` where :math:`y = x + \frac{1}{x}`

     :math:`\therefore y = \frac{-(a - 1)\pm \sqrt{(a - 1)^2 + 4}}{2}`

     :math:`\Rightarrow x + \frac{1}{x} = \frac{-(a - 1)\pm \sqrt{(a - 1)^2 + 4}}{2}`

     :math:`2x^2 + [(a - 1) - \sqrt{(a - 1)^2 + 4}]x + 2 = 0` and

     :math:`2x^2 + [(a - 1) + \sqrt{(a - 1)^2 + 4}]x + 2 = 0` are two equations we have.

     Let :math:`\alpha, \beta` are roots for first and :math:`\gamma, \delta` are roots
     for second.

     :math:`\therefore \alpha + \beta = -\frac{[(a - 1) - \sqrt{(a - 1)^2 +4}]}{2}` and :math:`\alpha\beta = 1`

     :math:`\therefore \gamma + \delta = -\frac{[(a - 1) + \sqrt{(a - 1)^2 +4}]}{2}` and :math:`\gamma\delta = 1`

     :math:`\because \sqrt{(a - 1)^2 + 4}> a - 1`

     :math:`\alpha + \beta > 0` and :math:`\alpha\beta > 0` hence both roots cannot be negative.

     Thus, :math:`\gamma` and :math:`\delta` have to be negative as per requirement from question.
     They have to be real and distinct because :math:`\gamma + \delta < 0` and :math:`\gamma\delta >0`
     do not imply that :math:`\gamma<0` and :math:`\delta < 0`.

     For both these to be negative discriminant has to be positive.

     Thus, :math:`[(a - 1) + \sqrt{(a - 1)^2 + 4}] - 16 > 0`

     Solving this we get :math:`\frac{5}{2}<a<\infty`

324. This problem is similar as last one and has been left as an exercise.

325. Given system of equations can be written as:

     :math:`ax_1^2 + (b - 1)x_1 + c = x_2 - x_1`

     :math:`ax_2^2 + (b - 1)x_2 + c = x_3 - x_2`

     :math:`\ldots`

     :math:`ax_n^2 + (b - 1)x_n + c = x_1 - x_n`

     Let :math:`f(x) = ax^2 + (b - 1)x + c` then we have

     :math:`f(x_1) = x_2 - x_1`

     :math:`f(x_2) = x_3 - x_2`

     :math:`\ldots`

     :math:`f(x_n) = x_1 - x_n`

     Case I: When :math:`(b - 1)^2 - 4ac < 0`:

     In this case all of :math:`f(x_1), f(x_2), \ldots, f(x_n)` will have same sign
     as that of :math:`a`.

     :math:`\therefore f(x_1) + f(x_2) + \ldots + f(x_n) \ne 0.`

     Hence, the system of equation have no solution.

     Case II: When :math:`(b - 1)^2 - 4ac = 0`

     In this case all of :math:`f(x_1), f(x_2), \ldots, f(x_n) \ge 0` or
     :math:`f(x_1), f(x_2), \ldots, f(x_n) \le 0`

     But :math:`f(x_1) + f(x_2) + \ldots + f(x_n) = 0` implies

     :math:`f(x_1) = f(x_2) = \ldots = f(x_n) = 0`

     Then, we have :math:`f(x_k)=0\Rightarrow ax_k^2 + (b - 1)x_k + c = 0`

     :math:`\Rightarrow x_k = \frac{1 - b}{2a}`

     Case III: When :math:`(b - 1)^2 - 4ac > 0:`

     Roots are :math:`\alpha,\beta = \frac{1 - b + \sqrt{(1 - b)^2 - 4ac}}{2a}`

     Now it is trivial to find rest from sign scheme.

326. This inequality is system of two inequalities. First we do one.

     i. :math:`x^2 - \frac{3}{16} > 0 \Rightarrow x < -\frac{\sqrt{3}}{4}` or :math:`x > \frac{\sqrt{3}}{4}`

     ii. :math:`x > 1`

     iii. :math:`x^2 - \frac{3}{16}> x^4 \Rightarrow 16x^4 - 16x^2 + 3 < 0`

          :math:`(4x^2 -3)(4x^2 - 1) < 0 \Rightarrow \frac{1}{4}<x^2\frac{3}{4}`

          :math:`x^2 > \frac{1}{4} \Rightarrow x < -\frac{1}{2}` or :math:`x > \frac{1}{2}`

          and :math:`x^2 < \frac{3}{4} \Rightarrow -\frac{\sqrt{3}}{2}< x < \frac{\sqrt{3}}{2}`

     Second system of inequality is left as an exercise.

327. Given :math:`\log_{\frac{1}{2}}x^2 \ge \log_{\frac{1}{2}}(x + 2)`

     :math:`\Rightarrow x^2 \le x + 2` [ :math:`\because` base :math:`< 1` ]

     :math:`\Rightarrow x^2 - x - 2 \le 0`

     :math:`\Rightarrow -1 \le x \le 2, x \ne 0`

     [For logarithms to be defined :math:`x\ne 0` and :math:`x>-2`]

     Again, :math:`49x^2 - 4m^4 < 0`

     :math:`-\frac{2}{7}m^2\le x \le \frac{2}{7}m^2`

     According to question :math:`[-1, 2] \subset \left[-\frac{2}{7}m^2, \frac{2}{7}m^2\right]`

     Now it is trivial to solve for various values of :math:`m` which reader can compute to be
     :math:`-\infty<m \le -\sqrt{7}` or :math:`\sqrt{7}\le m < \infty` 

328. Given, :math:`1 + \log_5(x^2 + 1)\geq \log_5(ax^2 + 4x + a)`

     :math:`\Leftrightarrow \log_55 + \log_5(x^2 + 1)\geq \log_5(ax^2 + 4x + a)`

     :math:`\Leftrightarrow \log_55(x^2 + 1)\geq \log_5(ax^2 + 4x + a)`

     :math:`\Leftrightarrow 5(x^2 + 1)\geq ax^2 + 4x + a`

     :math:`\Leftrightarrow (5 - a)x^2 - 4x + 5 -a \geq 0~~\forall` real :math:`x`

     i. :math:`D\leq 0 \Leftrightarrow 16 - 4(5 - a)^2 \leq 0 \Leftrightarrow (7 - a)(a - 3)\leq 0`

        :math:`\Leftrightarrow a\leq 3` or :math:`a\geq 7`

     ii. :math:`5 - a > 0 \Leftrightarrow a < 5`

         Combining from (i) we have :math:`a\leq 3`

     iii. But for :math:`\log_5(ax^2 + 4x + a)` to be defined

          :math:`ax^2 + 4x + a > 0~\forall` real :math:`x`

          :math:`D < 0 \Leftrightarrow 16 - 4a^2 < 0 \Leftrightarrow a < -2` or :math:`a > 2`

          and :math:`a > 0`

          Combining from (ii) we have :math:`2 < a \leq 3`

329. Let :math:`a - c = \alpha, b - c = \beta` and :math:`c + x = u` then for :math:`\sqrt{a - c}` and
     and :math:`\sqrt{b - c}` to be real :math:`\alpha \geq 0` and :math:`\beta \geq 0`. Also as,
     :math:`x > -c \therefore u > 0`

     Let :math:`y = \frac{(a + x)(b + x)}{c + x} = \frac{(u + \alpha)(u + \beta)}{u}`

     :math:`y = u + \frac{\alpha\beta}{u} + \alpha + \beta`

     :math:`u^2 + (\alpha + \beta - y)u + \alpha\beta = 0`

     Since :math:`u` is real :math:`\therefore (\alpha + \beta - y)^2 - 4\alpha\beta \geq 0`

     :math:`y^2 -2(\alpha + \beta)y + (\alpha - \beta)^2 \geq 0`

     Roots are :math:`y = (\sqrt{\alpha} - \sqrt{\beta})^2, (\sqrt{\alpha} + \sqrt{\beta})^2`

     :math:`y \leq (\sqrt{\alpha} - \sqrt{\beta})^2` and :math:`y \geq (\sqrt{\alpha} + \sqrt{\beta})^2`

     But :math:`y \leq (\sqrt{\alpha} - \sqrt{\beta})^2 \Leftrightarrow y - (\alpha + \beta) +
     2\sqrt{\alpha\beta}\leq 0` which is not possible as :math:`y - \alpha - \beta = u +
     \frac{\alpha\beta}{u}>0`

     Hence, least value of y = :math:`(\sqrt{a - c} + \sqrt{b - c})^2`

Rest of the problems have been left as exercise.
