.. meta::
   :author: Shiv Shankar Dayal
   :title: Quadratic Equations Solutions Part 5
   :description: Quadratic Equations Solutions Part 5
   :keywords: quadratic equations, algebra

Quadratic Equations Solutions Part 5
************************************
201. Product of roots :math:`= \frac{k + 2}{k} = \frac{c}{a}`

     :math:`\Rightarrow k = \frac{2a}{c - a}`

     Sum of roots :math:`= \frac{k + 1}{k} + \frac{k + 2}{k + 1} = -\frac{b}{a}`

     Substituting for :math:`k`

     :math:`\frac{c + a}{2a} + \frac{2c}{c + a} = - \frac{b}{a}`

     :math:`\frac{(a + c)^2 + 4ac}{2a(a + c)} = -\frac{b}{a}`

     :math:`a(a + c)^2 + 4a^2c = -2abc - 2a^2b`

     :math:`(a + c)^2 + 4ac = -2bc - 2ab`

     :math:`(a + b + c)^2 = b^2 - 4ac`
202. Given, :math:`f(x) = ax^2 + bx + c` and that :math:`\alpha,\beta` are the roots of the equation :math:`px^2 + qx +
     r = 0`

     :math:`\alpha + \beta = -\frac{q}{p}` and :math:`\alpha\beta = \frac{r}{p}`

     Now :math:`f(\alpha)f(\beta) = (a\alpha^2 + b\alpha + c)(a\beta^2 + b\beta + c)`

     :math:`= a^2\alpha^2\beta^2 + b^2\alpha\beta + c^2 + ab\alpha\beta(\alpha + \beta) + ac(\alpha^2 + \beta^2) +
     bc(\alpha + \beta)`

     :math:`= a^2\frac{r^2}{p^2} + b^2\frac{r}{p} + c^2 - ab\frac{r}{p}\frac{q}{p} + ac\left(\frac{q^2}{p^2} -
     \frac{2r}{p}\right) - bc\frac{q}{p}`

     :math:`= \frac{1}{p^2}[a^2r^2 + b^2rp + c^2p^2 - abrq + acq^2 - 2acrp - bcqp]`

     :math:`= \frac{1}{p^2}[(cp - ar)^2 + b^2rp - bcqp - abrq + acq^2]`

     :math:`= \frac{1}{p^2}[(cp - ar)^2 - (bp - aq)(cq - br)]`

     Now since :math:`\alpha, \beta` are the roots of the equation :math:`px^2 + qx + r = 0`

     Therefore, if :math:`ax^2 + bx + c = 0` and :math:`px^2 + qx + r = 0` have to have a common root then it has to be
     either :math:`\alpha` or :math:`\beta`.

     :math:`f(\alpha) = 0` or :math:`f(\beta) = 0 \therefore f(\alpha)f(\beta) = 0`

     :math:`\Rightarrow (cp - ar)^2 - (bp - aq)(cq - br) = 0`

     :math:`\therefore bp - aq, cp - ar, cq - br` are in G. P.
203. From the given equations it follows that :math:`q` and :math:`r` are roots of the equation

     :math:`a(p + x)^2 + 2bpx + c = 0 \Rightarrow ax^2 + 2(a + b)px + c = 0`

     Product of roots :math:`qr = \frac{ap^2 + c}{a} = p^2 + \frac{c}{a}`
204. Since :math:`\alpha, \beta` are the roots of the equation :math:`x^2 - px - (p + c) = 0`

     :math:`\alpha + \beta = p` and :math:`\alpha + \beta = -(p + c)`

     Now :math:`(\alpha + 1)(\beta + 1) = -p - c + p + 1 = 1 - c`

     :math:`\frac{\alpha^2 + 2\alpha + 1}{\alpha^2 + 2\alpha + c} + \frac{\beta^2 + 2\beta + 1}{\beta^2 + 2\beta + c} =
     \frac{(\alpha + 1)^2}{(\alpha + 1)^2 - (1 - c) + \frac{(\beta + 1)^2}{(\beta + 1)^2 - (1 - c)}}`

     :math:`= \frac{(\alpha + 1)^2}{(\alpha + 1)^2 - (\alpha + 1)(\beta + 1) + \frac{(\beta + 1)^2}{(\beta + 1)^2 -
     (\alpha 1)(\beta + 1)}}`

     :math:`= \frac{(\alpha + 1)^2}{(\alpha + 1)(\alpha - \beta)} + \frac{(\beta + 1)^2}{(\beta + 1)(\alpha - \beta)} =
     1`
205. :math:`\alpha, \beta` are the roots of the equation :math:`x^2 + px + q = 0`

     :math:`\therefore \alpha + \beta = -p` and :math:`\alpha\beta = q`

     Since :math:`\alpha, \beta` are the roots of the equation :math:`x^2{2n} + p^nx^n + q^n = 0`

     Substituting it follows that :math:`\alpha^n, \beta^n` are the roots of the equation :math:`y^2 + p^ny + q^n = 0`

     :math:`\therefore \alpha^n + \beta^n = -p^n` and :math:`\alpha^n\beta^n = q^n`

     :math:`(\alpha + \beta)^n = (-p)^n = p^n [\because~\text{n is even}]`

     Thus, :math:`\alpha^n + \beta^n + (\alpha + \beta)^n = 0`

     Dividing by :math:`\beta^n` we have

     :math:`\left(\frac{\alpha}{\beta}\right)^n + 1 + \left(\frac{\alpha}{\beta} + 1\right)^n = 0`

     Dividing by :math:`\alpha^n` we have

     :math:`\left(\frac{\beta}{\alpha}\right)^n + 1 + \left(\frac{\beta}{\alpha} + 1\right)^n = 0`

     From last two equations it is evident that :math:`\frac{\alpha}{\beta}` and :math:`\frac{\beta}{\alpha}` are roots
     of the equation :math:`x^n + 1 + (x + 1)^n = 0`
206. Following from previous problem: :math:`\alpha^n + \beta^n = -p^n`

     Also since :math:`\frac{\alpha}{\beta}` and :math:`\frac{\beta}{\alpha}` are roots
     of the equation :math:`x^n + 1 + (x + 1)^n = 0`

     :math:`\alpha^n + \beta^n = -(\alpha + \beta)^n = -(-p)^n`

     From these equations we have :math:`-p^n = -(-p)^n \Rightarrow p^n = (-p)^n`

     Therefore, :math:`n` must be even.
207. Let :math:`\alpha` and :math:`\beta` are the roots of the given equation.

     Since roots are real and distinct :math:`D > 0 \Rightarrow a^2 - 4b > 0 \Rightarrow b < \frac{a^2}{4}`

     Again it is given that :math:`|\alpha - \beta| < c \Rightarrow (\alpha - \beta)^2 < c^2`

     :math:`(\alpha + \beta)^2 - 4\alpha\beta < c^2 \Rightarrow a^2 - 4b < c^2 \Rightarrow 4b > a^2 - c^2`

     :math:`\Rightarrow \frac{a^2 - c^2}{4} < b < \frac{a^2}{4}`
208. Given, :math:`ax^2 + bx + c - p = 0` for two integral values of :math:`x` say :math:`\alpha` and :math:`\beta`.

     Then, :math:`\alpha + \beta = -\frac{b}{a}` and :math:`\alpha\beta = \frac{c - p}{a}`

     If possible, let :math:`ax^2 + bx + c - 2p = 0` for some integer :math:`k`.

     :math:`ak^2 + bk + c - p = p \Rightarrow k^2 - (\alpha + \beta)k + \alpha\beta = \frac{p}{a}`

     :math:`(k - \alpha)(k - \beta) =~\text{an integer}~= \frac{p}{a}`

     But since :math:`p` is prime this cannot hold true unless :math:`a = p` or :math:`a = 1`

     :math:`a = p [\because a > 1]`

     :math:`(k - \alpha)(k - \beta) = 1` which implies that :math:`k - \alpha = k - \beta = 1`

     which is not possible since :math:`\alpha \ne \beta`

     Thus, we have a contradiction. Hence, :math:`ax^2 + bx + c \ne 2p` for any integral value of :math:`x`.
209. :math:`\alpha + \beta = -p, \alpha\beta = q, \alpha^4 + \beta^4 = r, \alpha^4\beta^4 = s`

     Let :math:`D` be the discriminant of :math:`x^2 - 4qx + 2q^2 - r = 0` then

     :math:`D = 16q^2 - 4(2q^2 - r) = 8q^2 + 4r = 8\alpha^2\beta^2 + 4(\alpha^4 + \beta^4) = 4(\alpha^2 + \beta^2)^2`

     :math:`D \ge 0` hence roots of the third equation are always real.
210. :math:`\alpha + \beta = -\frac{b}{a}` and :math:`\alpha\beta = \frac{c}{a}`

     :math:`\alpha_1 - \beta = -\frac{b_1}{a_1}` and :math:`-\alpha_1\beta = \frac{c_1}{a_1}`

     :math:`\alpha + \alpha_1 = -\left(\frac{b}{a} + \frac{b_1}{a_1}\right)`

     Also, dividing :math:`\alpha + \beta` by :math:`\alpha\beta`

     :math:`\frac{1}{\beta} + \frac{1}{\alpha} = -\frac{b}{c}`

     Similarly, dividing :math:`\alpha_1 - \beta` by :math:`-\alpha_1\beta`

     :math:`\frac{1}{\alpha_1} - \frac{1}{\beta} = -\frac{b_1}{c_1}`

     Thus, :math:`\frac{1}{\alpha} + \frac{1}{\alpha_1} = -\left(\frac{b}{c} + \frac{b_1}{c_1}\right)`

     Equation whose roots are :math:`\alpha` and :math:`\alpha_1` is

     :math:`x^2 - (\alpha + \alpha_1)x + \alpha\alpha_1 = 0`

     :math:`\frac{x^2}{-(\alpha + \alpha_1)} + x - \frac{\alpha\alpha_1}{\alpha + \alpha_1} = 0`

     :math:`\frac{x^2}{\frac{b}{a} + \frac{b_1}{a_1}} + x + \frac{1}{\frac{b}{c} + \frac{b_1}{c_1}} = 0`
211. Let :math:`\alpha` and :math:`\beta` be roots of such quadratic equation given by :math:`x^2 + px + q = 0`

     :math:`\alpha + \beta = -p` and :math:`\alpha\beta = q`

     Now quadratic equation whose roots are :math:`\alpha^2` and :math:`\beta^2` is

     :math:`x^2 - (\alpha^2 + \beta^2)x + \alpha^2\beta^2 = 0`

     :math:`x^2 - (p^2 - 2q)x + q^2 = 0`

     But the equation remains unchanged, therefore,

     :math:`\frac{1}{1} = \frac{p}{p^2 - 2q} = \frac{q}{q^2}`

     :math:`\Rightarrow q = q^2 \Rightarrow q(q - 1) = 0 \Rightarrow q = 0, 1`

     If :math:`q = 0 \Rightarrow p = 0, -1`

     and if :math:`q = 1 \Rightarrow p = -2, 1`

     Thus, four such quadratic equations are possible.
212. Given :math:`\frac{d}{a}, \frac{e}{b}, \frac{f}{c}` are in A. P. and :math:`a, b, c` are in G. P.

     Equations :math:`ax^2 + 2bx + c = 0` and :math:`dx^2 + 2ex + f = 0` will have a common root if

     :math:`\frac{2(bf - ec)}{cd - af} = \frac{cd - af}{2(ae - bd)}`

     :math:`4(bf - ec)(ae - bd) = (cd - af)^2`

     :math:`4\left[\left(\frac{f}{c} - \frac{e}{b}\right)bc\right]\left[\left(\frac{e}{b} - \frac{d}{a}\right)ab\right]
     = \left(\frac{d}{a} - \frac{a}{f}\right)^2a^2c^2`

     :math:`4k.k.b^2 = 4k^2ac` where :math:`k` is the c.d. of the A. P.

     :math:`b^2 = ac` which is true because :math:`a, b, c` are in G. P.
213. Let :math:`\alpha` be the common root and :math:`\beta_1` another root of :math:`x^2 + ax + 12 = 0, \beta_2` be
     another root of :math:`x^2 + bx + 15 = 0` and :math:`\beta_3` be a root of :math:`x^2 + (a + b)x + 36 = 0.`

     :math:`\alpha + \beta_1 = -a` and :math:`\alpha\beta_1 = 12`

     :math:`\alpha + \beta_2 = -b` and :math:`\alpha\beta_2 = 15`

     :math:`\alpha + \beta_3 = -(a + b)` and :math:`\alpha\beta_3 = 36`

     Thus, :math:`2\alpha + \beta_1 + \beta_2 = \alpha + \beta_3 \Rightarrow \alpha = \beta_3 - \beta_1 - \beta_2`

     and :math:`\alpha(\beta_3 - \beta_1 - \beta_2) = 36 - 12 - 15 = 9`

     :math:`\Rightarrow \alpha^2 = 9 \Rightarrow \alpha = \pm 3` but :math:`\alpha > 0 \Rightarrow \alpha = 3`

     :math:`\Rightarrow \beta_1 = 4, \beta_2 = 5, \beta_3 = 12`
214. Given :math:`m(ax^2 + 2bx + c) + px^2 + 1qx + r = n(x + k)^2`

     Equating coefficients for powers of :math:`x`, we get

     :math:`ma + p = n, mb + q = nk, mc + r = nk^2`

     :math:`\Rightarrow m(ak - b) + pk - q = 0 \Rightarrow m = -\frac{pk - q}{ak - b}`

     :math:`\Rightarrow m(bk - c) + qk - r = 0 \Rightarrow m = -\frac{qk - r}{bk - c}`

     Equating values for :math:`m`

     :math:`(ak - b)(qk - r) = (pk - q)(bk - c)`
215. Given equation is :math:`x^3 - x^2 + \beta x + \gamma = 0`

     Let it roots :math:`x_1, x_2, x_3` be :math:`a - d, a, a + d` respectively.

     :math:`a - d + a + a + d = 1 \Rightarrow a = \frac{1}{3}`

     :math:`(a - d)a + a(a + d) + (a - d)(a + d) = \beta \Rightarrow 3a^2 - d^2 = \beta \Rightarrow 1 - 3\beta = 3d^2`

     :math:`(a - d)a(a + d) = \gamma \Rightarrow a(a^2 - d^2) = \gamma \Rightarrow 1 + 27\gamma = 9d^2`

     Since :math:`d` is real :math:`\therefore 1 - 3\beta \ge 0 \Rightarrow \beta \le \frac{1}{3}`

     :math:`1 + 27\gamma \ge 0 \Rightarrow \gamma \ge -\frac{1}{27}`
216. Let :math:`\alpha` be a common root, then

     :math:`\alpha^3 + 3p\alpha^2 + 3q\alpha + r = 0` ... (1) and :math:`\alpha^2 + 2p\alpha + q = 0` ... (2)

     :math:`(1) - \alpha (2)` gives us :math:`\Rightarrow p\alpha^2 + 2q\alpha + r = 0` ... (3)

     By cross multiplication between (2) and (3)

     :math:`\frac{\alpha^2}{2(pr - q^2)} = \frac{\alpha}{pq - r} = \frac{1}{2(q - p^2)}`

     Equating for values of :math:`\alpha` we get the desired condition.
217. Let :math:`\alpha` be a common root, then

     :math:`\alpha^3 + 2a\alpha^2 + 3b\alpha + c = 0` ... (1) and :math:`\alpha^3 + a\alpha^2 + 2b\alpha = 0` ... (2)

     Since :math:`c \ne 0,` therefore :math:`\alpha = 0` cannot be a common root. Therefore, from (2)

     :math:`\alpha^2 + a\alpha + 2b = 0` ... (3)

     :math:`(1) - \alpha (2) \Rightarrow a\alpha^2 + b\alpha + c = 0` ... (4)

     Solving (3) and (4) by cross-multiplication yields the desired result.
218. Given equation is :math:`x^3 + ax + b = 0` and :math:`\alpha, \beta, \gamma` be its real roots. Then we have

     :math:`\alpha + \beta + \gamma = 0` ... (1) :math:`\alpha\beta + \beta\gamma + \alpha\gamma = a` ... (2)
     :math:`\alpha\beta\gamma = -b`

     Let :math:`y = (\alpha - \beta)^2,` then :math:`y = (\alpha + \beta)^2 - 4\alpha\beta`

     :math:`y = \gamma^2 + \frac{4b}{\gamma}` :math:`\Rightarrow \gamma^3 - y\gamma + 4b = 0`

     Also, :math:`\gamma` is a root of the original equation.

     :math:`\gamma^3 + a\gamma + b = 0`

     :math:`(a + y)\gamma - 3b = 0 \Rightarrow \gamma = \frac{3b}{a + y}`

     :math:`\Rightarrow \frac{27b^3}{(a + y)^3} + a\left(\frac{3b}{a + y}\right) + b = 0`

     :math:`y^3 + 6ay^2 + 9a^2y + 4a^3 + 27b^2 = 0`

     We will get same equation if we would have chosen :math:`y = (\beta - \alpha)^2` or :math:`y = (\gamma - \alpha)^2`

     Hence, product of roots :math:`-(4a^3 + 27b^2) = (\alpha - \beta)^2(\beta - \gamma)^2(\gamma - \alpha)^2 \ge 0`

     :math:`\therefore 4a^3 + 27b^2 \le 0`
