Solutions for Proportions
*************************
1. a. Let the number is x. Then, we have,

.. math::
   \frac{3}{4}=\frac{9}{x}~
   \Rightarrow~x=12

Second and third part are left as exercise to the reader.

2. a. Let mean proportional be x so we have,

.. math::
   x^2=ab~\Rightarrow~x=\sqrt{ab}

Second part is left as an exercise.

3. a. Let third proportional be x. Then, we have,

.. math::
   9^2=7x~\Rightarrow~x=\frac{81}{7}

Second part is left as an exercise.

4. a. Let us equate the given proportion\'s ratios to k.

.. math::
   \frac{a}{b}=\frac{c}{d}~\Rightarrow~a=bk,~c=dk

Now let us evaluate L.H.S. by substituing above value for a and c.

.. math::
   \frac{a^c+ac^2}{b^d+bd^2}=\frac{b^2k^2dk+bkd^2k^2}{b^d+db^2}=k^3

Now let us evaluate R.H.S. by substituing above value for a and c.

.. math::
   \frac{(bk+dk)^3}{(b+d)^3}=k^3

.. math::
   \text{Hence,} L.H.S.= R.H.S.

5. Proceeding the same way as previous problem we have L.H.S. as

.. math::
   \frac{pb^2k^2+qb^2}{p^2k^2-qb^2}=\frac{pk^2+q}{pk^2-q}

and R.H.S. as

.. math::
   \frac{pd^2k^2+qd^2}{pd^2k^2-qd^2}=\frac{pk^2+q}{pk^2-q}

.. math::
   \text{Hence,} L.H.S.= R.H.S.

6. Processing similarly L.H.S. is

.. math::
   \frac{bk-dk}{b-d}=k

and R.H.S. is

.. math::
   \frac{\sqrt{b^2k^2+d^2k^2}}{\sqrt{b^2+d^2}} = k

.. math::
   \text{Hence,} L.H.S.= R.H.S.

7. We have computed R.H.S. to be k in last problem\'s R.H.S. So let us try to
calculate R.H.S.

.. math::
   \frac{\sqrt{bdk^2+\frac{d^3k^3}{bk}}}{\sqrt{bd+\frac{d^3}{b}}}=k

8. Since a, b, c and d are in continued proportion we can write them as

.. math::
   \frac{a}{b}=\frac{b}{c}=\frac{c}{d}=k

.. math::
   \Rightarrow~a=dk^3, b=dk^2,~\text{and}~c=dk

First we do L.H.S.

.. math::
   \frac{a}{b+d}=\frac{dk^3}{dk^2+d}=\frac{k^3}{k^2+1}

now we do R.H.S.

.. math::
   \frac{c^3}{c^2d+d^3}=\frac{d^3k^3}{d^2k^2d+d^2}=\frac{k^3}{k^2+1}.

Problem no. 9 and 10 are left as exercises to the reader as they are similar.

11. Since b is mean proportional between a and b we can write
:math:`b^2=ac`. Now let us evaluate the expression.

.. math::
   L.H.S.=\frac{a^2-ac+c^2}{\frac{1}{a^2}-\frac{1}{ac}+\frac{1}{c^2}}
